@prefix IAO: <http://purl.obolibrary.org/obo/IAO_> .
@prefix NCIT: <http://ncicb.nci.nih.gov/xml/owl/EVS/Thesaurus.owl#> .
@prefix OIO: <http://www.geneontology.org/formats/oboInOwl#> .
@prefix bibo: <http://purl.org/ontology/bibo/> .
@prefix dcterms: <http://purl.org/dc/terms/> .
@prefix linkml: <https://w3id.org/linkml/> .
@prefix oslc: <http://open-services.net/ns/core#> .
@prefix owl: <http://www.w3.org/2002/07/owl#> .
@prefix pav: <http://purl.org/pav/> .
@prefix prov: <http://www.w3.org/ns/prov#> .
@prefix qb: <http://purl.org/linked-data/cube#> .
@prefix qudt: <http://qudt.org/schema/qudt/> .
@prefix rdf: <http://www.w3.org/1999/02/22-rdf-syntax-ns#> .
@prefix rdfs: <http://www.w3.org/2000/01/rdf-schema#> .
@prefix schema: <http://schema.org/> .
@prefix sh: <http://www.w3.org/ns/shacl#> .
@prefix skos: <http://www.w3.org/2004/02/skos/core#> .
@prefix skosxl: <http://www.w3.org/2008/05/skos-xl#> .
@prefix swrl: <http://www.w3.org/2003/11/swrl#> .
@prefix vann: <https://vocab.org/vann/> .
@prefix xsd: <http://www.w3.org/2001/XMLSchema#> .

linkml:equals_number_in a owl:ObjectProperty,
        linkml:SlotDefinition ;
    rdfs:label "equals_number_in" ;
    rdfs:range linkml:Integer ;
    rdfs:subPropertyOf linkml:list_value_specification_constant ;
    skos:definition "the slot must have range number and the value of the slot must equal one of the specified values" .

linkml:inapplicable a owl:ObjectProperty,
        linkml:SlotDefinition ;
    rdfs:label "inapplicable" ;
    rdfs:domain linkml:SlotDefinition ;
    rdfs:range linkml:Boolean ;
    skos:definition "true means that values for this slot must not be present" ;
    skos:note "By default all slots are applicable. The main use case for this slot is as an override in a subclass" .

linkml:inlined_as_simple_dict a owl:ObjectProperty,
        linkml:SlotDefinition ;
    rdfs:label "inlined_as_simple_dict" ;
    rdfs:domain linkml:SlotDefinition ;
    rdfs:range linkml:Boolean ;
    rdfs:seeAlso "https://w3id.org/linkml/docs/specification/06mapping/#collection-forms" ;
    skos:definition "True means that an inlined slot is represented as a simple dict whose values are all atoms" .

linkml:meta a owl:Ontology ;
    rdfs:label "meta" ;
    IAO:0000700 linkml:AltDescription,
        linkml:Annotatable,
        linkml:Anything,
        linkml:ClassExpression,
        linkml:ClassLevelRule,
        linkml:CommonMetadata,
        linkml:Example,
        linkml:Expression,
        linkml:Extensible,
        linkml:Extension,
        linkml:LocalName,
        linkml:MatchQuery,
        linkml:Prefix,
        linkml:ReachabilityQuery,
        linkml:Setting,
        linkml:UnitOfMeasure ;
    dcterms:license "https://creativecommons.org/publicdomain/zero/1.0/" ;
    dcterms:title "LinkML Schema Metamodel" ;
    pav:version "2.0.0" ;
    linkml:generation_date "2023-03-16T10:58:30" ;
    linkml:metamodel_version "1.7.0" ;
    linkml:source_file "meta.yaml" ;
    linkml:source_file_date "2023-03-11T19:19:30" ;
    linkml:source_file_size 89120 .

linkml:owned_by a owl:ObjectProperty,
        linkml:SlotDefinition ;
    rdfs:label "owned_by" ;
    rdfs:domain linkml:Element ;
    rdfs:range linkml:Uriorcurie ;
    skos:altLabel "owner",
        "steward" ;
    skos:closeMatch rdfs:isDefinedBy ;
    skos:definition "agent that owns or is the steward of the element" .

linkml:structured_imports a owl:ObjectProperty,
        linkml:SlotDefinition ;
    rdfs:label "structured_imports" ;
    rdfs:domain linkml:SchemaDefinition ;
    rdfs:range linkml:ImportExpression ;
    skos:definition "A list of specifications for how to import elements from external schemas" .

linkml:topValue a owl:DatatypeProperty ;
    rdfs:label "value" .

linkml:value_specification_constant a owl:ObjectProperty,
        linkml:SlotDefinition ;
    rdfs:label "value_specification_constant" ;
    rdfs:range linkml:String ;
    skos:definition "Grouping for metamodel slots that constrain the a slot value to equal a specified constant" .

dcterms:contributor a owl:ObjectProperty,
        linkml:SlotDefinition ;
    rdfs:label "contributors" ;
    rdfs:domain linkml:Element ;
    rdfs:range linkml:Uriorcurie ;
    skos:definition "agent that contributed to the element" ;
    skos:exactMatch dcterms:contributor .

dcterms:publisher a owl:ObjectProperty,
        linkml:SlotDefinition ;
    rdfs:label "publisher" ;
    rdfs:domain linkml:Element ;
    rdfs:range linkml:Uriorcurie ;
    skos:definition "An entity responsible for making the resource available" ;
    skos:exactMatch dcterms:publisher .

linkml:abstract a owl:ObjectProperty,
        linkml:SlotDefinition ;
    rdfs:label "abstract" ;
    rdfs:domain linkml:Definition ;
    rdfs:range linkml:Boolean ;
    skos:definition "Indicates the class or slot cannot be directly instantiated and is intended for grouping purposes." .

linkml:asymmetric a owl:ObjectProperty,
        linkml:SlotDefinition ;
    rdfs:label "asymmetric" ;
    rdfs:domain linkml:SlotDefinition ;
    rdfs:range linkml:Boolean ;
    rdfs:subPropertyOf linkml:relational_logical_characteristic ;
    skos:closeMatch owl:AsymmetricProperty ;
    skos:definition "If s is antisymmetric, and i.s=v where i is different from v, v.s cannot have value i" ;
    skos:note "asymmetry is the combination of antisymmetry and irreflexivity" .

linkml:attributes a owl:ObjectProperty,
        linkml:SlotDefinition ;
    rdfs:label "attributes" ;
    rdfs:domain linkml:ClassDefinition ;
    rdfs:range linkml:SlotDefinition ;
    skos:definition "Inline definition of slots" ;
    skos:note "attributes are an alternative way of defining new slots.  An attribute adds a slot to the global space in the form <class_name>__<slot_name> (lower case, double underscores).  Attributes can be specialized via slot_usage." .

linkml:base a owl:ObjectProperty,
        linkml:SlotDefinition ;
    rdfs:label "base" ;
    rdfs:domain linkml:TypeDefinition ;
    rdfs:range linkml:String ;
    skos:definition "python base type in the LinkML runtime that implements this type definition" ;
    skos:note "every root type must have a base",
        "the base is inherited by child types but may be overriden.  Base compatibility is not checked." .

linkml:bidirectional a owl:ObjectProperty,
        linkml:SlotDefinition ;
    rdfs:label "bidirectional" ;
    rdfs:range linkml:Boolean ;
    skos:altLabel "if and only if",
        "iff" ;
    skos:definition "in addition to preconditions entailing postconditions, the postconditions entail the preconditions" .

linkml:class_uri a owl:ObjectProperty,
        linkml:SlotDefinition ;
    rdfs:label "class_uri" ;
    rdfs:domain linkml:ClassDefinition ;
    rdfs:range linkml:Uriorcurie ;
    rdfs:seeAlso "https://linkml.io/linkml/schemas/uris-and-mappings.html",
        "linkml:definition_uri" ;
    skos:altLabel "public ID" ;
    skos:definition "URI of the class that provides a semantic interpretation of the element in a linked data context. The URI may come from any namespace and may be shared between schemas" ;
    skos:note "Assigning class_uris can provide additional hooks for interoperation, indicating a common conceptual model" .

linkml:classes a owl:ObjectProperty,
        linkml:SlotDefinition ;
    rdfs:label "classes" ;
    rdfs:domain linkml:SchemaDefinition ;
    rdfs:range linkml:ClassDefinition ;
    skos:definition "An index to the collection of all class definitions in the schema" .

linkml:classification_rules a owl:ObjectProperty,
        linkml:SlotDefinition ;
    rdfs:label "classification_rules" ;
    rdfs:domain linkml:ClassDefinition ;
    rdfs:range linkml:AnonymousClassExpression ;
    skos:definition "The collection of classification rules that apply to all members of this class. Classification rules allow for automatically assigning the instantiated type of an instance." .

linkml:consider_nulls_inequal a owl:ObjectProperty,
        linkml:SlotDefinition ;
    rdfs:label "consider_nulls_inequal" ;
    rdfs:domain linkml:UniqueKey ;
    rdfs:range linkml:Boolean ;
    skos:definition "By default, None values are considered equal for the purposes of comparisons in determining uniqueness. Set this to true to treat missing values as per ANSI-SQL NULLs, i.e NULL=NULL is always False." .

linkml:default_curi_maps a owl:ObjectProperty,
        linkml:SlotDefinition ;
    rdfs:label "default_curi_maps" ;
    rdfs:domain linkml:SchemaDefinition ;
    rdfs:range linkml:String ;
    skos:definition "ordered list of prefixcommon biocontexts to be fetched to resolve id prefixes and inline prefix variables" .

linkml:default_prefix a owl:ObjectProperty,
        linkml:SlotDefinition ;
    rdfs:label "default_prefix" ;
    rdfs:domain linkml:SchemaDefinition ;
    rdfs:range linkml:String ;
    skos:definition "The prefix that is used for all elements within a schema" .

linkml:default_range a owl:ObjectProperty,
        linkml:SlotDefinition ;
    rdfs:label "default_range" ;
    rdfs:domain linkml:SchemaDefinition ;
    rdfs:range linkml:TypeDefinition ;
    skos:definition "default slot range to be used if range element is omitted from a slot definition" .

linkml:defining_slots a owl:ObjectProperty,
        linkml:SlotDefinition ;
    rdfs:label "defining_slots" ;
    rdfs:domain linkml:ClassDefinition ;
    rdfs:range linkml:SlotDefinition ;
    skos:definition "The combination of is a plus defining slots form a genus-differentia definition, or the set of necessary and sufficient conditions that can be transformed into an OWL equivalence axiom" .

linkml:definition_uri a owl:ObjectProperty,
        linkml:SlotDefinition ;
    rdfs:label "definition_uri" ;
    rdfs:domain linkml:Element ;
    rdfs:range linkml:Uriorcurie ;
    rdfs:seeAlso "linkml:class_uri",
        "linkml:slot_uri" ;
    skos:definition "The native URI of the element. This is always within the namespace of the containing schema. Contrast with the assigned URI, via class_uri or slot_uri" ;
    skos:note "Formed by combining the default_prefix with the normalized element name" .

linkml:derivation a owl:ObjectProperty,
        linkml:SlotDefinition ;
    rdfs:label "derivation" ;
    rdfs:range linkml:String ;
    skos:definition "Expression for deriving this unit from other units" .

linkml:designates_type a owl:ObjectProperty,
        linkml:SlotDefinition ;
    rdfs:label "designates_type" ;
    rdfs:domain linkml:SlotDefinition ;
    rdfs:range linkml:Boolean ;
    rdfs:seeAlso "https://linkml.io/linkml/schemas/type-designators.html" ;
    skos:altLabel "type designator" ;
    skos:definition "True means that the key slot(s) is used to determine the instantiation (types) relation between objects and a ClassDefinition" .

linkml:domain a owl:ObjectProperty,
        linkml:SlotDefinition ;
    rdfs:label "domain" ;
    rdfs:domain linkml:SlotDefinition ;
    rdfs:range linkml:ClassDefinition ;
    skos:definition """defines the type of the subject of the slot.  Given the following slot definition
  S1:
    domain: C1
    range:  C2
the declaration
  X:
    S1: Y

implicitly asserts that X is an instance of C1
""" .

linkml:domain_of a owl:ObjectProperty,
        linkml:SlotDefinition ;
    rdfs:label "domain_of" ;
    rdfs:domain linkml:SlotDefinition ;
    rdfs:range linkml:ClassDefinition ;
    skos:definition "the class(es) that reference the slot in a \"slots\" or \"slot_usage\" context" ;
    skos:exactMatch schema:domainIncludes .

linkml:elseconditions a owl:ObjectProperty,
        linkml:SlotDefinition ;
    rdfs:label "elseconditions" ;
    rdfs:range linkml:AnonymousClassExpression ;
    rdfs:seeAlso "https://w3id.org/linkml/docs/specification/05validation/#rules" ;
    skos:altLabel "else" ;
    skos:definition "an expression that must hold for an instance of the class, if the preconditions no not hold" .

linkml:emit_prefixes a owl:ObjectProperty,
        linkml:SlotDefinition ;
    rdfs:label "emit_prefixes" ;
    rdfs:domain linkml:SchemaDefinition ;
    rdfs:range linkml:Ncname ;
    skos:definition "a list of Curie prefixes that are used in the representation of instances of the model.  All prefixes in this list are added to the prefix sections of the target models." .

linkml:enum_uri a owl:ObjectProperty,
        linkml:SlotDefinition ;
    rdfs:label "enum_uri" ;
    rdfs:domain linkml:EnumDefinition ;
    rdfs:range linkml:Uriorcurie ;
    skos:altLabel "public ID" ;
    skos:definition "URI of the enum that provides a semantic interpretation of the element in a linked data context. The URI may come from any namespace and may be shared between schemas" .

linkml:enums a owl:ObjectProperty,
        linkml:SlotDefinition ;
    rdfs:label "enums" ;
    rdfs:domain linkml:SchemaDefinition ;
    rdfs:range linkml:EnumDefinition ;
    skos:definition "An index to the collection of all enum definitions in the schema" .

linkml:followed_by a owl:ObjectProperty,
        linkml:SlotDefinition ;
    rdfs:label "followed_by" ;
    rdfs:range linkml:Expression ;
    skos:definition "in a sequential list, this indicates the next member" .

linkml:generation_date a owl:ObjectProperty,
        linkml:SlotDefinition ;
    rdfs:label "generation_date" ;
    rdfs:domain linkml:SchemaDefinition ;
    rdfs:range linkml:Datetime ;
    skos:definition "date and time that the schema was loaded/generated" .

linkml:id a owl:ObjectProperty,
        linkml:SlotDefinition ;
    rdfs:label "id" ;
    rdfs:domain linkml:SchemaDefinition ;
    rdfs:range linkml:Uri ;
    skos:definition "The official schema URI" .

linkml:id_prefixes a owl:ObjectProperty,
        linkml:SlotDefinition ;
    rdfs:label "id_prefixes" ;
    rdfs:domain linkml:Element ;
    rdfs:range linkml:Ncname ;
    rdfs:seeAlso "https://github.com/linkml/linkml-model/issues/28",
        "https://github.com/linkml/linkml/issues/194" ;
    skos:definition "An allowed list of prefixes for which identifiers must conform. The identifier of this class or slot must begin with the URIs referenced by this prefix" ;
    skos:note "If identifiers are treated as CURIEs, then the CURIE must start with one of the indicated prefixes followed by `:` (_should_ start if the list is open)",
        "If identifiers are treated as URIs, then the URI string must start with the expanded for of the prefix (_should_ start if the list is open)",
        "Order of elements may be used to indicate priority order" .

linkml:identifier a owl:ObjectProperty,
        linkml:SlotDefinition ;
    rdfs:label "identifier" ;
    rdfs:domain linkml:SlotDefinition ;
    rdfs:range linkml:Boolean ;
    rdfs:seeAlso "https://en.wikipedia.org/wiki/Identifier",
        "linkml:unique_keys" ;
    skos:altLabel "ID",
        "UID",
        "code",
        "primary key" ;
    skos:definition "True means that the key slot(s) uniquely identifies the elements. There can be at most one identifier or key per container" ;
    skos:note "a given domain can have at most one identifier",
        "a key slot is automatically required.  Identifiers cannot be optional",
        "identifier is inherited",
        "identifiers and keys are mutually exclusive.  A given domain cannot have both" .

linkml:identifier_pattern a owl:ObjectProperty,
        linkml:SlotDefinition ;
    rdfs:label "identifier_pattern" ;
    rdfs:domain linkml:MatchQuery ;
    rdfs:range linkml:String ;
    skos:definition "A regular expression that is used to obtain a set of identifiers from a source_ontology to construct a set of permissible values" .

linkml:ifabsent a owl:ObjectProperty,
        linkml:SlotDefinition ;
    rdfs:label "ifabsent" ;
    rdfs:domain linkml:SlotDefinition ;
    rdfs:range linkml:String ;
    rdfs:seeAlso "linkml:equals_expression" ;
    skos:closeMatch sh:defaultValue ;
    skos:definition """function that provides a default value for the slot.  Possible values for this slot are defined in
linkml.utils.ifabsent_functions.default_library:
  * [Tt]rue -- boolean True
  * [Ff]alse -- boolean False
  * bnode -- blank node identifier
  * class_curie -- CURIE for the containing class
  * class_uri -- URI for the containing class
  * default_ns -- schema default namespace
  * default_range -- schema default range
  * int(value) -- integer value
  * slot_uri -- URI for the slot
  * slot_curie -- CURIE for the slot
  * string(value) -- string value""" .

linkml:implements a owl:ObjectProperty,
        linkml:SlotDefinition ;
    rdfs:label "implements" ;
    rdfs:domain linkml:Element ;
    rdfs:range linkml:Uriorcurie ;
    skos:definition "An element in another schema which this element conforms to. The referenced element is not imported into the schema for the implementing element. However, the referenced schema may be used to check conformance of the implementing element." .

linkml:import_as a owl:ObjectProperty,
        linkml:SlotDefinition ;
    rdfs:label "import_as" ;
    rdfs:domain linkml:ImportExpression ;
    rdfs:range linkml:Ncname .

linkml:import_from a owl:ObjectProperty,
        linkml:SlotDefinition ;
    rdfs:label "import_from" ;
    rdfs:domain linkml:ImportExpression ;
    rdfs:range linkml:Uriorcurie .

linkml:import_map a owl:ObjectProperty,
        linkml:SlotDefinition ;
    rdfs:label "import_map" ;
    rdfs:domain linkml:ImportExpression ;
    rdfs:range linkml:Setting .

linkml:imports a owl:ObjectProperty,
        linkml:SlotDefinition ;
    rdfs:label "imports" ;
    rdfs:domain linkml:SchemaDefinition ;
    rdfs:range linkml:Uriorcurie ;
    skos:definition "A list of schemas that are to be included in this schema" .

linkml:include_self a owl:ObjectProperty,
        linkml:SlotDefinition ;
    rdfs:label "include_self" ;
    rdfs:domain linkml:ReachabilityQuery ;
    rdfs:range linkml:Boolean ;
    skos:altLabel "reflexive" ;
    skos:definition "True if the query is reflexive" .

linkml:inherited a owl:ObjectProperty,
        linkml:SlotDefinition ;
    rdfs:label "inherited" ;
    rdfs:domain linkml:SlotDefinition ;
    rdfs:range linkml:Boolean ;
    skos:definition "true means that the *value* of a slot is inherited by subclasses" ;
    skos:note "Inherited applies to slot values.  Parent *slots* are always inherited by subclasses",
        "the slot is to be used for defining *metamodels* only" .

linkml:interpolated a owl:ObjectProperty,
        linkml:SlotDefinition ;
    rdfs:label "interpolated" ;
    rdfs:domain linkml:PatternExpression ;
    rdfs:range linkml:Boolean ;
    skos:definition "if true then the pattern is first string interpolated" .

linkml:irreflexive a owl:ObjectProperty,
        linkml:SlotDefinition ;
    rdfs:label "irreflexive" ;
    rdfs:domain linkml:SlotDefinition ;
    rdfs:range linkml:Boolean ;
    rdfs:subPropertyOf linkml:relational_logical_characteristic ;
    skos:closeMatch owl:IrreflexiveProperty ;
    skos:definition "If s is irreflexive, then there exists no i such i.s=i" .

linkml:is_class_field a owl:ObjectProperty,
        linkml:SlotDefinition ;
    rdfs:label "is_class_field" ;
    rdfs:domain linkml:SlotDefinition ;
    rdfs:range linkml:Boolean ;
    skos:definition "indicates that for any instance, i, the domain of this slot will include an assertion of i s range" .

linkml:is_direct a owl:ObjectProperty,
        linkml:SlotDefinition ;
    rdfs:label "is_direct" ;
    rdfs:domain linkml:ReachabilityQuery ;
    rdfs:range linkml:Boolean ;
    skos:altLabel "non-transitive" ;
    skos:definition "True if the reachability query should only include directly related nodes, if False then include also transitively connected" .

linkml:is_grouping_slot a owl:ObjectProperty,
        linkml:SlotDefinition ;
    rdfs:label "is_grouping_slot" ;
    rdfs:domain linkml:SlotDefinition ;
    rdfs:range linkml:Boolean ;
    skos:closeMatch sh:PropertyGroup ;
    skos:definition "true if this slot is a grouping slot" .

linkml:is_usage_slot a owl:ObjectProperty,
        linkml:SlotDefinition ;
    rdfs:label "is_usage_slot" ;
    rdfs:domain linkml:SlotDefinition ;
    rdfs:range linkml:Boolean ;
    skos:definition "True means that this slot was defined in a slot_usage situation" .

linkml:key a owl:ObjectProperty,
        linkml:SlotDefinition ;
    rdfs:label "key" ;
    rdfs:domain linkml:SlotDefinition ;
    rdfs:range linkml:Boolean ;
    rdfs:seeAlso "linkml:unique_keys" ;
    skos:definition "True means that the key slot(s) uniquely identify the elements within a single container" ;
    skos:note "a given domain can have at most one key slot (restriction to be removed in the future)",
        "a key slot is automatically required.  Keys cannot be optional",
        "identifiers and keys are mutually exclusive.  A given domain cannot have both",
        "key is inherited" .

linkml:list_elements_ordered a owl:ObjectProperty,
        linkml:SlotDefinition ;
    rdfs:label "list_elements_ordered" ;
    rdfs:domain linkml:SlotDefinition ;
    rdfs:range linkml:Boolean ;
    skos:definition "If True, then the order of elements of a multivalued slot is guaranteed to be preserved. If False, the order may still be preserved but this is not guaranteed" ;
    skos:note "should only be used with multivalued slots" .

linkml:list_elements_unique a owl:ObjectProperty,
        linkml:SlotDefinition ;
    rdfs:label "list_elements_unique" ;
    rdfs:domain linkml:SlotDefinition ;
    rdfs:range linkml:Boolean ;
    skos:definition "If True, then there must be no duplicates in the elements of a multivalued slot" ;
    skos:note "should only be used with multivalued slots" .

linkml:local_name_source a owl:ObjectProperty,
        linkml:SlotDefinition ;
    rdfs:label "local_name_source" ;
    rdfs:domain linkml:LocalName ;
    rdfs:range linkml:Ncname ;
    skos:definition "the ncname of the source of the name" .

linkml:local_names a owl:ObjectProperty,
        linkml:SlotDefinition ;
    rdfs:label "local_names" ;
    rdfs:domain linkml:Element ;
    rdfs:range linkml:LocalName .

linkml:locally_reflexive a owl:ObjectProperty,
        linkml:SlotDefinition ;
    rdfs:label "locally_reflexive" ;
    rdfs:domain linkml:SlotDefinition ;
    rdfs:range linkml:Boolean ;
    rdfs:subPropertyOf linkml:relational_logical_characteristic ;
    skos:definition "If s is locally_reflexive, then i.s=i for all instances i where s is a class slot for the type of i" .

linkml:meaning a owl:ObjectProperty,
        linkml:SlotDefinition ;
    rdfs:label "meaning" ;
    rdfs:domain linkml:PermissibleValue ;
    rdfs:range linkml:Uriorcurie ;
    rdfs:seeAlso "https://en.wikipedia.org/wiki/ISO/IEC_11179" ;
    skos:altLabel "PV meaning" ;
    skos:definition "the value meaning of a permissible value" ;
    skos:editorialNote "we may want to change the range of this (and other) elements in the model to an entitydescription type construct" .

linkml:metamodel_version a owl:ObjectProperty,
        linkml:SlotDefinition ;
    rdfs:label "metamodel_version" ;
    rdfs:domain linkml:SchemaDefinition ;
    rdfs:range linkml:String ;
    skos:definition "Version of the metamodel used to load the schema" .

linkml:multivalued a owl:ObjectProperty,
        linkml:SlotDefinition ;
    rdfs:label "multivalued" ;
    rdfs:domain linkml:SlotDefinition ;
    rdfs:range linkml:Boolean ;
    skos:definition "true means that slot can have more than one value and should be represented using a list or collection structure." .

linkml:object a owl:ObjectProperty,
        linkml:SlotDefinition ;
    rdfs:label "object" ;
    rdfs:domain linkml:Example ;
    rdfs:range linkml:Anything ;
    skos:definition "direct object representation of the example" .

linkml:open_world a owl:ObjectProperty,
        linkml:SlotDefinition ;
    rdfs:label "open_world" ;
    rdfs:range linkml:Boolean ;
    skos:definition "if true, the the postconditions may be omitted in instance data, but it is valid for an inference engine to add these" .

linkml:owner a owl:ObjectProperty,
        linkml:SlotDefinition ;
    rdfs:label "owner" ;
    rdfs:domain linkml:SlotDefinition ;
    rdfs:range linkml:Definition ;
    skos:definition "the \"owner\" of the slot. It is the class if it appears in the slots list, otherwise the declaring slot" .

linkml:partial_match a owl:ObjectProperty,
        linkml:SlotDefinition ;
    rdfs:label "partial_match" ;
    rdfs:domain linkml:PatternExpression ;
    rdfs:range linkml:Boolean ;
    skos:definition "if true then the pattern must match the whole string, as if enclosed in ^...$" .

linkml:path_rule a owl:ObjectProperty,
        linkml:SlotDefinition ;
    rdfs:label "path_rule" ;
    rdfs:domain linkml:SlotDefinition ;
    rdfs:range linkml:PathExpression ;
    skos:definition "a rule for inferring a slot assignment based on evaluating a path through a sequence of slot assignemnts" .

linkml:postconditions a owl:ObjectProperty,
        linkml:SlotDefinition ;
    rdfs:label "postconditions" ;
    rdfs:range linkml:AnonymousClassExpression ;
    rdfs:seeAlso "https://w3id.org/linkml/docs/specification/05validation/#rules" ;
    skos:altLabel "consequents",
        "head",
        "then" ;
    skos:closeMatch swrl:body ;
    skos:definition "an expression that must hold for an instance of the class, if the preconditions hold" .

linkml:readonly a owl:ObjectProperty,
        linkml:SlotDefinition ;
    rdfs:label "readonly" ;
    rdfs:domain linkml:SlotDefinition ;
    rdfs:range linkml:String ;
    skos:definition "If present, slot is read only.  Text explains why" ;
    skos:note "the slot is to be used for defining *metamodels* only" .

linkml:reflexive a owl:ObjectProperty,
        linkml:SlotDefinition ;
    rdfs:label "reflexive" ;
    rdfs:domain linkml:SlotDefinition ;
    rdfs:range linkml:Boolean ;
    rdfs:subPropertyOf linkml:relational_logical_characteristic ;
    skos:closeMatch owl:ReflexiveProperty ;
    skos:definition "If s is reflexive, then i.s=i for all instances i" ;
    skos:note "it is rare for a property to be reflexive, this characteristic is added for completeness, consider instead locally_reflexive" .

linkml:reflexive_transitive_form_of a owl:ObjectProperty,
        linkml:SlotDefinition ;
    rdfs:label "reflexive_transitive_form_of" ;
    rdfs:range linkml:SlotDefinition ;
    rdfs:subPropertyOf linkml:transitive_form_of ;
    skos:definition "transitive_form_of including the reflexive case" .

linkml:relational_role a owl:ObjectProperty,
        linkml:SlotDefinition ;
    rdfs:label "relational_role" ;
    rdfs:domain linkml:SlotDefinition ;
    rdfs:range linkml:RelationalRoleEnum ;
    skos:altLabel "reification_role" ;
    skos:definition "the role a slot on a relationship class plays, for example, the subject, object or predicate roles" ;
    skos:note "in the context of RDF, this should be used for slots that can be modeled using the RDF reification vocabulary",
        "in the context of property graphs, this should be used on edge classes to indicate which slots represent the input and output nodes",
        "this should only be used on slots that are applicable to class that represent relationships" .

linkml:relationship_types a owl:ObjectProperty,
        linkml:SlotDefinition ;
    rdfs:label "relationship_types" ;
    rdfs:domain linkml:ReachabilityQuery ;
    rdfs:range linkml:Uriorcurie ;
    skos:altLabel "predicates",
        "properties" ;
    skos:definition "A list of relationship types (properties) that are used in a reachability query" .

linkml:repr a owl:ObjectProperty,
        linkml:SlotDefinition ;
    rdfs:label "repr" ;
    rdfs:domain linkml:TypeDefinition ;
    rdfs:range linkml:String ;
    skos:definition "the name of the python object that implements this type definition" .

linkml:represents_relationship a owl:ObjectProperty,
        linkml:SlotDefinition ;
    rdfs:label "represents_relationship" ;
    rdfs:domain linkml:ClassDefinition ;
    rdfs:range linkml:Boolean ;
    rdfs:seeAlso "https://patterns.dataincubator.org/book/qualified-relation.html",
        "rdf:Statement" ;
    skos:altLabel "is_reified" ;
    skos:definition "true if this class represents a relationship rather than an entity" ;
    skos:note "in the context of Entity-Relationship (ER) modeling, this is used to state that a class models a relationship between entities, and should be drawn with a diamond",
        "in the context of RDF, this should be used when instances of the class are `rdf:Statement`s",
        "in the context of property graphs, this should be used when a class is used to represent an edge that connects nodes" .

linkml:reversed a owl:ObjectProperty,
        linkml:SlotDefinition ;
    rdfs:label "reversed" ;
    rdfs:range linkml:Boolean ;
    skos:definition "true if the slot is to be inversed" .

linkml:role a owl:ObjectProperty,
        linkml:SlotDefinition ;
    rdfs:label "role" ;
    rdfs:domain linkml:SlotDefinition ;
    rdfs:range linkml:String ;
    skos:definition "a textual descriptor that indicates the role played by the slot range" ;
    skos:note "the primary use case for this slot is to provide a textual descriptor of a generic slot name when used in the context of a more specific class" .

linkml:setting_key a owl:ObjectProperty,
        linkml:SlotDefinition ;
    rdfs:label "setting_key" ;
    rdfs:domain linkml:Setting ;
    rdfs:range linkml:Ncname ;
    skos:definition "the variable name for a setting" .

linkml:setting_value a owl:ObjectProperty,
        linkml:SlotDefinition ;
    rdfs:label "setting_value" ;
    rdfs:domain linkml:Setting ;
    rdfs:range linkml:String ;
    skos:definition "The value assigned for a setting" .

linkml:settings a owl:ObjectProperty,
        linkml:SlotDefinition ;
    rdfs:label "settings" ;
    rdfs:domain linkml:SchemaDefinition ;
    rdfs:range linkml:Setting ;
    skos:altLabel "constants" ;
    skos:definition "A collection of global variable settings" ;
    skos:note "global variables are used in string interpolation in structured patterns" .

linkml:shared a owl:ObjectProperty,
        linkml:SlotDefinition ;
    rdfs:label "shared" ;
    rdfs:domain linkml:SlotDefinition ;
    rdfs:range linkml:Boolean ;
    skos:altLabel "inverse functional",
        "many to one or many" ;
    skos:definition "If True, then the relationship between the slot domain and range is many to one or many to many" .

linkml:singular_name a owl:ObjectProperty,
        linkml:SlotDefinition ;
    rdfs:label "singular_name" ;
    rdfs:domain linkml:SlotDefinition ;
    rdfs:range linkml:String ;
    skos:closeMatch skos:altLabel ;
    skos:definition "a name that is used in the singular form" ;
    skos:note "this may be used in some schema translations where use of a singular form is idiomatic, for example RDF" .

linkml:slot_uri a owl:ObjectProperty,
        linkml:SlotDefinition ;
    rdfs:label "slot_uri" ;
    rdfs:domain linkml:SlotDefinition ;
    rdfs:range linkml:Uriorcurie ;
    rdfs:seeAlso "https://linkml.io/linkml/schemas/uris-and-mappings.html",
        "linkml:definition_uri" ;
    skos:altLabel "public ID" ;
    skos:definition "URI of the class that provides a semantic interpretation of the slot in a linked data context. The URI may come from any namespace and may be shared between schemas." ;
    skos:note "Assigning slot_uris can provide additional hooks for interoperation, indicating a common conceptual model" .

linkml:slot_usage a owl:ObjectProperty,
        linkml:SlotDefinition ;
    rdfs:label "slot_usage" ;
    rdfs:domain linkml:ClassDefinition ;
    rdfs:range linkml:SlotDefinition ;
    skos:definition "the refinement of a slot in the context of the containing class definition." ;
    skos:note "Many slots may be re-used across different classes, but the meaning of the slot may be refined by context. For example, a generic association model may use slots subject/predicate/object with generic semantics and minimal constraints. When this is subclasses, e.g. to disease-phenotype associations then slot usage may specify both local naming (e.g. subject=disease) and local constraints" .

linkml:source_file a owl:ObjectProperty,
        linkml:SlotDefinition ;
    rdfs:label "source_file" ;
    rdfs:domain linkml:SchemaDefinition ;
    rdfs:range linkml:String ;
    skos:definition "name, uri or description of the source of the schema" .

linkml:source_file_date a owl:ObjectProperty,
        linkml:SlotDefinition ;
    rdfs:label "source_file_date" ;
    rdfs:domain linkml:SchemaDefinition ;
    rdfs:range linkml:Datetime ;
    skos:definition "modification date of the source of the schema" .

linkml:source_file_size a owl:ObjectProperty,
        linkml:SlotDefinition ;
    rdfs:label "source_file_size" ;
    rdfs:domain linkml:SchemaDefinition ;
    rdfs:range linkml:Integer ;
    skos:definition "size in bytes of the source of the schema" .

linkml:source_nodes a owl:ObjectProperty,
        linkml:SlotDefinition ;
    rdfs:label "source_nodes" ;
    rdfs:domain linkml:ReachabilityQuery ;
    rdfs:range linkml:Uriorcurie ;
    skos:definition "A list of nodes that are used in the reachability query" .

linkml:string_serialization a owl:ObjectProperty,
        linkml:SlotDefinition ;
    rdfs:label "string_serialization" ;
    rdfs:domain linkml:Definition ;
    rdfs:range linkml:String ;
    rdfs:seeAlso "https://github.com/linkml/issues/128" ;
    skos:definition """Used on a slot that stores the string serialization of the containing object. The syntax follows python formatted strings, with slot names enclosed in {}s. These are expanded using the values of those slots.
We call the slot with the serialization the s-slot, the slots used in the {}s are v-slots. If both s-slots and v-slots are populated on an object then the value of the s-slot should correspond to the expansion.
Implementations of frameworks may choose to use this property to either (a) PARSE: implement automated normalizations by parsing denormalized strings into complex objects (b) GENERARE: implement automated to_string labeling of complex objects
For example, a Measurement class may have 3 fields: unit, value, and string_value. The string_value slot may have a string_serialization of {value}{unit} such that if unit=cm and value=2, the value of string_value shouldd be 2cm""" .

linkml:subclass_of a owl:ObjectProperty,
        linkml:SlotDefinition ;
    rdfs:label "subclass_of" ;
    rdfs:domain linkml:ClassDefinition ;
    rdfs:range linkml:Uriorcurie ;
    skos:closeMatch rdfs:subClassOf ;
    skos:definition "DEPRECATED -- rdfs:subClassOf to be emitted in OWL generation" .

linkml:subsets a owl:ObjectProperty,
        linkml:SlotDefinition ;
    rdfs:label "subsets" ;
    rdfs:domain linkml:SchemaDefinition ;
    rdfs:range linkml:SubsetDefinition ;
    skos:definition "An index to the collection of all subset definitions in the schema" ;
    skos:exactMatch OIO:hasSubset .

linkml:symmetric a owl:ObjectProperty,
        linkml:SlotDefinition ;
    rdfs:label "symmetric" ;
    rdfs:domain linkml:SlotDefinition ;
    rdfs:range linkml:Boolean ;
    rdfs:subPropertyOf linkml:relational_logical_characteristic ;
    skos:closeMatch owl:SymmetricProperty ;
    skos:definition "If s is symmetric, and i.s=v, then v.s=i" .

linkml:syntax a owl:ObjectProperty,
        linkml:SlotDefinition ;
    rdfs:label "syntax" ;
    rdfs:domain linkml:PatternExpression ;
    rdfs:range linkml:String ;
    skos:definition "the string value of the slot must conform to this regular expression expressed in the string. May be interpolated." .

linkml:tag a owl:ObjectProperty,
        linkml:SlotDefinition ;
    rdfs:label "tag" ;
    rdfs:domain linkml:Extension ;
    rdfs:range linkml:Uriorcurie ;
    skos:definition "a tag associated with an extension" .

linkml:text a owl:ObjectProperty,
        linkml:SlotDefinition ;
    rdfs:label "text" ;
    rdfs:domain linkml:PermissibleValue ;
    rdfs:range linkml:String ;
    skos:altLabel "value" ;
    skos:closeMatch skos:notation ;
    skos:definition "The actual permissible value itself" ;
    skos:note "there are no constraints on the text of the permissible value, but for many applications you may want to consider following idiomatic forms and using computer-friendly forms" .

linkml:transitive a owl:ObjectProperty,
        linkml:SlotDefinition ;
    rdfs:label "transitive" ;
    rdfs:domain linkml:SlotDefinition ;
    rdfs:range linkml:Boolean ;
    rdfs:subPropertyOf linkml:relational_logical_characteristic ;
    skos:closeMatch owl:TransitiveProperty ;
    skos:definition "If s is transitive, and i.s=z, and s.s=j, then i.s=j" .

linkml:traverse a owl:ObjectProperty,
        linkml:SlotDefinition ;
    rdfs:label "traverse" ;
    rdfs:range linkml:SlotDefinition ;
    skos:definition "the slot to traverse" .

linkml:traverse_up a owl:ObjectProperty,
        linkml:SlotDefinition ;
    rdfs:label "traverse_up" ;
    rdfs:domain linkml:ReachabilityQuery ;
    rdfs:range linkml:Boolean ;
    skos:altLabel "ancestors" ;
    skos:definition "True if the direction of the reachability query is reversed and ancestors are retrieved" .

linkml:tree_root a owl:ObjectProperty,
        linkml:SlotDefinition ;
    rdfs:label "tree_root" ;
    rdfs:domain linkml:ClassDefinition ;
    rdfs:range linkml:Boolean ;
    rdfs:seeAlso "https://linkml.io/linkml/intro/tutorial02.html" ;
    skos:definition "Indicates that this is the Container class which forms the root of the serialized document structure in tree serializations" ;
    skos:editorialNote "each schema should have at most one tree root" .

linkml:typeof a owl:ObjectProperty,
        linkml:SlotDefinition ;
    rdfs:label "typeof" ;
    rdfs:domain linkml:TypeDefinition ;
    rdfs:range linkml:TypeDefinition ;
    skos:definition "A parent type from which type properties are inherited" ;
    skos:note "the target type definition of the typeof slot is referred to as the \"parent type\"",
        "the type definition containing the typeof slot is referred to as the \"child type\"",
        "type definitions without a typeof slot are referred to as a \"root type\"" .

linkml:types a owl:ObjectProperty,
        linkml:SlotDefinition ;
    rdfs:label "types" ;
    rdfs:domain linkml:SchemaDefinition ;
    rdfs:range linkml:TypeDefinition ;
    skos:definition "An index to the collection of all type definitions in the schema" .

linkml:unique_key_name a owl:ObjectProperty,
        linkml:SlotDefinition ;
    rdfs:label "unique_key_name" ;
    rdfs:domain linkml:UniqueKey ;
    rdfs:range linkml:String ;
    skos:definition "name of the unique key" .

linkml:unique_keys a owl:ObjectProperty,
        linkml:SlotDefinition ;
    rdfs:label "unique_keys" ;
    rdfs:domain linkml:ClassDefinition ;
    rdfs:range linkml:UniqueKey ;
    rdfs:seeAlso "https://linkml.io/linkml/schemas/constraints.html#unique-key" ;
    skos:definition "A collection of named unique keys for this class. Unique keys may be singular or compound." ;
    skos:exactMatch owl:hasKey .

linkml:uri a owl:ObjectProperty,
        linkml:SlotDefinition ;
    rdfs:label "uri" ;
    rdfs:domain linkml:TypeDefinition ;
    rdfs:range linkml:Uriorcurie ;
    skos:definition "The uri that defines the possible values for the type definition" ;
    skos:note "every root type must have a type uri",
        "uri is typically drawn from the set of URI's defined in OWL (https://www.w3.org/TR/2012/REC-owl2-syntax-20121211/#Datatype_Maps)" .

linkml:usage_slot_name a owl:ObjectProperty,
        linkml:SlotDefinition ;
    rdfs:label "usage_slot_name" ;
    rdfs:domain linkml:SlotDefinition ;
    rdfs:range linkml:String ;
    skos:definition "The name of the slot referenced in the slot_usage" .

linkml:values_from a owl:ObjectProperty,
        linkml:SlotDefinition ;
    rdfs:label "values_from" ;
    rdfs:domain linkml:Definition ;
    rdfs:range linkml:Uriorcurie ;
    skos:definition "The identifier of a \"value set\" -- a set of identifiers that form the possible values for the range of a slot. Note: this is different than 'subproperty_of' in that 'subproperty_of' is intended to be a single ontology term while 'values_from' is the identifier of an entire value set.  Additionally, this is different than an enumeration in that in an enumeration, the values of the enumeration are listed directly in the model itself. Setting this property on a slot does not guarantee an expansion of the ontological hiearchy into an enumerated list of possible values in every serialization of the model." .

dcterms:conformsTo a owl:ObjectProperty,
        linkml:SlotDefinition ;
    rdfs:label "conforms_to" ;
    rdfs:domain linkml:Element ;
    rdfs:range linkml:String ;
    rdfs:seeAlso "linkml:implements" ;
    skos:definition "An established standard to which the element conforms." ;
    skos:exactMatch dcterms:conformsTo .

dcterms:license a owl:ObjectProperty,
        linkml:SlotDefinition ;
    rdfs:label "license" ;
    rdfs:domain linkml:SchemaDefinition ;
    rdfs:range linkml:String ;
    skos:definition "license for the schema" ;
    skos:exactMatch dcterms:license .

pav:version a owl:ObjectProperty,
        linkml:SlotDefinition ;
    rdfs:label "version" ;
    rdfs:domain linkml:SchemaDefinition ;
    rdfs:range linkml:String ;
    skos:definition "particular version of schema" ;
    skos:exactMatch pav:version,
        schema:schemaVersion .

qudt:abbreviation a owl:ObjectProperty,
        linkml:SlotDefinition ;
    rdfs:label "abbreviation" ;
    rdfs:range linkml:String ;
    skos:definition "An abbreviation for a unit is a short ASCII string that is used in place of the full name for the unit in contexts where non-ASCII characters would be problematic, or where using the abbreviation will enhance readability. When a power of a base unit needs to be expressed, such as squares this can be done using abbreviations rather than symbols (source: qudt)" ;
    skos:exactMatch qudt:abbreviation .

qudt:hasQuantityKind a owl:ObjectProperty,
        linkml:SlotDefinition ;
    rdfs:label "has_quantity_kind" ;
    rdfs:range linkml:Uriorcurie ;
    skos:definition "Concept in a vocabulary or ontology that denotes the kind of quanity being measured, e.g. length" ;
    skos:exactMatch qudt:hasQuantityKind ;
    skos:note "Potential ontologies include but are not limited to PATO, NCIT, OBOE, qudt.quantityKind" .

qudt:iec61360Code a owl:ObjectProperty,
        linkml:SlotDefinition ;
    rdfs:label "iec61360code" ;
    rdfs:range linkml:String ;
    skos:exactMatch qudt:iec61360Code .

qudt:symbol a owl:ObjectProperty,
        linkml:SlotDefinition ;
    rdfs:label "symbol" ;
    rdfs:range linkml:String ;
    skos:definition "name of the unit encoded as a symbol" ;
    skos:exactMatch qudt:symbol .

qudt:ucumCode a owl:ObjectProperty,
        linkml:SlotDefinition ;
    rdfs:label "ucum_code" ;
    rdfs:domain linkml:UnitOfMeasure ;
    rdfs:range linkml:String ;
    skos:definition "associates a QUDT unit with its UCUM code (case-sensitive)." ;
    skos:exactMatch qudt:ucumCode .

schema:keywords a owl:ObjectProperty,
        linkml:SlotDefinition ;
    rdfs:label "keywords" ;
    rdfs:domain linkml:Element ;
    rdfs:range linkml:String ;
    skos:definition "Keywords or tags used to describe the element" ;
    skos:exactMatch schema:keywords .

rdf:object a owl:Class,
        linkml:RelationalRoleEnum ;
    rdfs:label "OBJECT" .

rdf:subject a owl:Class,
        linkml:RelationalRoleEnum ;
    rdfs:label "SUBJECT" .

rdfs:subPropertyOf a owl:ObjectProperty,
        linkml:SlotDefinition ;
    rdfs:label "subproperty_of" ;
    rdfs:domain linkml:SlotDefinition ;
    rdfs:range linkml:SlotDefinition ;
    skos:definition "Ontology property which this slot is a subproperty of.  Note: setting this property on a slot does not guarantee an expansion of the ontological hiearchy into an enumerated list of possible values in every serialization of the model." ;
    skos:exactMatch rdfs:subPropertyOf ;
    linkml:examples "Example(value='RO:HOM0000001', description='this is the RO term for \"in homology relationship with\", and used as a value of subproperty of this means that any ontological child (related to RO:HOM0000001 via an is_a relationship), is a valid value for the slot that declares this with the subproperty_of tag.  This differs from the \\'values_from\\' meta model component in that \\'values_from\\' requires the id of a value set (said another way, if an entire ontology had a curie/identifier that was the identifier for the entire ontology, then that identifier would be used in \\'values_from.\\')')" .

owl:inverseOf a owl:ObjectProperty,
        linkml:SlotDefinition ;
    rdfs:label "inverse" ;
    rdfs:domain linkml:SlotDefinition ;
    rdfs:range linkml:SlotDefinition ;
    skos:definition "indicates that any instance of d s r implies that there is also an instance of r s' d" ;
    skos:exactMatch owl:inverseOf .

skos:broaderMatch a owl:Class,
        linkml:AliasPredicateEnum ;
    rdfs:label "BROAD_SYNONYM" .

skos:example a owl:ObjectProperty,
        linkml:SlotDefinition ;
    rdfs:label "value" ;
    rdfs:domain linkml:Example ;
    rdfs:range linkml:String ;
    skos:definition "example value" ;
    skos:exactMatch skos:example .

skos:narrowerMatch a owl:Class,
        linkml:AliasPredicateEnum ;
    rdfs:label "NARROW_SYNONYM" .

skos:prefLabel a owl:ObjectProperty,
        linkml:SlotDefinition ;
    rdfs:label "alias" ;
    rdfs:domain linkml:SlotDefinition ;
    rdfs:range linkml:String ;
    skos:definition "the name used for a slot in the context of its owning class.  If present, this is used instead of the actual slot name." ;
    skos:exactMatch skos:prefLabel ;
    skos:note "an example of alias is used within this metamodel, slot_definitions is aliases as slots",
        "not to be confused with aliases, which indicates a set of terms to be used for search purposes." .

skosxl:literalForm a owl:ObjectProperty,
        linkml:SlotDefinition ;
    rdfs:label "literal_form" ;
    rdfs:domain linkml:StructuredAlias ;
    rdfs:range linkml:String ;
    skos:altLabel "alias_name",
        "string_value" ;
    skos:definition "The literal lexical form of a structured alias; i.e the actual alias value." ;
    skos:exactMatch skosxl:literalForm .

sh:condition a owl:ObjectProperty,
        linkml:SlotDefinition ;
    rdfs:label "preconditions" ;
    rdfs:range linkml:AnonymousClassExpression ;
    rdfs:seeAlso "https://w3id.org/linkml/docs/specification/05validation/#rules" ;
    skos:altLabel "antecedents",
        "body",
        "if" ;
    skos:closeMatch swrl:body ;
    skos:definition "an expression that must hold in order for the rule to be applicable to an instance" ;
    skos:exactMatch sh:condition .

sh:deactivated a owl:ObjectProperty,
        linkml:SlotDefinition ;
    rdfs:label "deactivated" ;
    rdfs:range linkml:Boolean ;
    skos:definition "a deactivated rule is not executed by the rules engine" ;
    skos:exactMatch sh:deactivated .

sh:declare a owl:ObjectProperty,
        linkml:SlotDefinition ;
    rdfs:label "prefixes" ;
    rdfs:domain linkml:SchemaDefinition ;
    rdfs:range linkml:Prefix ;
    skos:definition "A collection of prefix expansions that specify how CURIEs can be expanded to URIs" ;
    skos:exactMatch sh:declare .

sh:group a owl:ObjectProperty,
        linkml:SlotDefinition ;
    rdfs:label "slot_group" ;
    rdfs:domain linkml:SlotDefinition ;
    rdfs:range linkml:SlotDefinition ;
    skos:definition "allows for grouping of related slots into a grouping slot that serves the role of a group" ;
    skos:exactMatch sh:group ;
    skos:note "slot groups do not change the semantics of a model but are a useful way of visually grouping related slots" .

sh:namespace a owl:ObjectProperty,
        linkml:SlotDefinition ;
    rdfs:label "prefix_reference" ;
    rdfs:domain linkml:Prefix ;
    rdfs:range linkml:Uri ;
    skos:definition "The namespace to which a prefix expands to." ;
    skos:exactMatch sh:namespace .

sh:prefix a owl:ObjectProperty,
        linkml:SlotDefinition ;
    rdfs:label "prefix_prefix" ;
    rdfs:domain linkml:Prefix ;
    rdfs:range linkml:Ncname ;
    skos:definition "The prefix components of a prefix expansions. This is the part that appears before the colon in a CURIE." ;
    skos:exactMatch sh:prefix .

sh:rule a owl:ObjectProperty,
        linkml:SlotDefinition ;
    rdfs:label "rules" ;
    rdfs:domain linkml:ClassDefinition ;
    rdfs:range linkml:ClassRule ;
    skos:definition "the collection of rules that apply to all members of this class" ;
    skos:exactMatch sh:rule .

linkml:AnonymousExpression a owl:Class,
        linkml:ClassDefinition ;
    rdfs:label "anonymous_expression" ;
    rdfs:subClassOf [ a owl:Restriction ;
            owl:maxQualifiedCardinality 1 ;
            owl:onClass linkml:Integer ;
            owl:onProperty sh:order ],
        [ a owl:Restriction ;
            owl:allValuesFrom linkml:Uriorcurie ;
            owl:onProperty skos:narrowMatch ],
        [ a owl:Restriction ;
            owl:maxQualifiedCardinality 1 ;
            owl:onClass linkml:Uriorcurie ;
            owl:onProperty linkml:deprecated_element_has_possible_replacement ],
        [ a owl:Restriction ;
            owl:maxQualifiedCardinality 1 ;
            owl:onClass linkml:Uriorcurie ;
            owl:onProperty pav:createdBy ],
        [ a owl:Restriction ;
            owl:maxQualifiedCardinality 1 ;
            owl:onClass linkml:Uriorcurie ;
            owl:onProperty linkml:deprecated_element_has_exact_replacement ],
        [ a owl:Restriction ;
            owl:allValuesFrom linkml:Uriorcurie ;
            owl:onProperty skos:mappingRelation ],
        [ a owl:Restriction ;
            owl:allValuesFrom linkml:StructuredAlias ;
            owl:onProperty skosxl:altLabel ],
        [ a owl:Restriction ;
            owl:allValuesFrom linkml:Uriorcurie ;
            owl:onProperty skos:broadMatch ],
        [ a owl:Restriction ;
            owl:maxQualifiedCardinality 1 ;
            owl:onClass linkml:Uriorcurie ;
            owl:onProperty oslc:modifiedBy ],
        [ a owl:Restriction ;
            owl:allValuesFrom linkml:Uriorcurie ;
            owl:onProperty skos:exactMatch ],
        [ a owl:Restriction ;
            owl:allValuesFrom linkml:AltDescription ;
            owl:onProperty linkml:alt_descriptions ],
        [ a owl:Restriction ;
            owl:allValuesFrom linkml:String ;
            owl:onProperty linkml:todos ],
        [ a owl:Restriction ;
            owl:allValuesFrom linkml:String ;
            owl:onProperty skos:altLabel ],
        [ a owl:Restriction ;
            owl:allValuesFrom linkml:String ;
            owl:onProperty skos:editorialNote ],
        [ a owl:Restriction ;
            owl:maxQualifiedCardinality 1 ;
            owl:onClass linkml:String ;
            owl:onProperty schema:inLanguage ],
        [ a owl:Restriction ;
            owl:allValuesFrom linkml:Example ;
            owl:onProperty linkml:examples ],
        [ a owl:Restriction ;
            owl:allValuesFrom linkml:Uriorcurie ;
            owl:onProperty skos:closeMatch ],
        [ a owl:Restriction ;
            owl:allValuesFrom linkml:Annotation ;
            owl:onProperty linkml:annotations ],
        [ a owl:Restriction ;
            owl:allValuesFrom linkml:Uriorcurie ;
            owl:onProperty rdfs:seeAlso ],
        [ a owl:Restriction ;
            owl:maxQualifiedCardinality 1 ;
            owl:onClass linkml:String ;
            owl:onProperty dcterms:title ],
        [ a owl:Restriction ;
            owl:maxQualifiedCardinality 1 ;
            owl:onClass linkml:String ;
            owl:onProperty skos:definition ],
        [ a owl:Restriction ;
            owl:allValuesFrom linkml:SubsetDefinition ;
            owl:onProperty OIO:inSubset ],
        [ a owl:Restriction ;
            owl:maxQualifiedCardinality 1 ;
            owl:onClass linkml:String ;
            owl:onProperty linkml:imported_from ],
        [ a owl:Restriction ;
            owl:maxQualifiedCardinality 1 ;
            owl:onClass linkml:Uriorcurie ;
            owl:onProperty dcterms:source ],
        [ a owl:Restriction ;
            owl:maxQualifiedCardinality 1 ;
            owl:onClass linkml:Datetime ;
            owl:onProperty pav:lastUpdatedOn ],
        [ a owl:Restriction ;
            owl:maxQualifiedCardinality 1 ;
            owl:onClass linkml:Uriorcurie ;
            owl:onProperty bibo:status ],
        [ a owl:Restriction ;
            owl:maxQualifiedCardinality 1 ;
            owl:onClass linkml:Datetime ;
            owl:onProperty pav:createdOn ],
        [ a owl:Restriction ;
            owl:allValuesFrom linkml:Extension ;
            owl:onProperty linkml:extensions ],
        [ a owl:Restriction ;
            owl:allValuesFrom linkml:String ;
            owl:onProperty skos:note ],
        [ a owl:Restriction ;
            owl:maxQualifiedCardinality 1 ;
            owl:onClass linkml:Uri ;
            owl:onProperty skos:inScheme ],
        [ a owl:Restriction ;
            owl:allValuesFrom linkml:Uriorcurie ;
            owl:onProperty skos:relatedMatch ],
        [ a owl:Restriction ;
            owl:maxQualifiedCardinality 1 ;
            owl:onClass linkml:String ;
            owl:onProperty linkml:deprecated ],
        linkml:Annotatable,
        linkml:CommonMetadata,
        linkml:Expression,
        linkml:Extensible ;
    skos:definition "An abstract parent class for any nested expression" ;
    skos:note "anonymous expressions are useful for when it is necessary to build a complex expression without introducing a named element for each sub-expression" .

linkml:ClassLevelRule a owl:Class,
        linkml:ClassDefinition ;
    rdfs:label "class_level_rule" ;
    skos:definition "A rule that is applied to classes" .

linkml:ClassRule a owl:Class,
        linkml:ClassDefinition ;
    rdfs:label "class_rule" ;
    rdfs:subClassOf [ a owl:Restriction ;
            owl:maxQualifiedCardinality 1 ;
            owl:onClass linkml:Uriorcurie ;
            owl:onProperty linkml:deprecated_element_has_possible_replacement ],
        [ a owl:Restriction ;
            owl:maxQualifiedCardinality 1 ;
            owl:onClass linkml:Uriorcurie ;
            owl:onProperty dcterms:source ],
        [ a owl:Restriction ;
            owl:allValuesFrom linkml:Uriorcurie ;
            owl:onProperty rdfs:seeAlso ],
        [ a owl:Restriction ;
            owl:allValuesFrom linkml:String ;
            owl:onProperty skos:note ],
        [ a owl:Restriction ;
            owl:allValuesFrom linkml:Uriorcurie ;
            owl:onProperty skos:mappingRelation ],
        [ a owl:Restriction ;
            owl:maxQualifiedCardinality 1 ;
            owl:onClass linkml:Uriorcurie ;
            owl:onProperty pav:createdBy ],
        [ a owl:Restriction ;
            owl:allValuesFrom linkml:String ;
            owl:onProperty linkml:todos ],
        [ a owl:Restriction ;
            owl:maxQualifiedCardinality 1 ;
            owl:onClass linkml:String ;
            owl:onProperty skos:definition ],
        [ a owl:Restriction ;
            owl:maxQualifiedCardinality 1 ;
            owl:onClass linkml:String ;
            owl:onProperty schema:inLanguage ],
        [ a owl:Restriction ;
            owl:allValuesFrom linkml:Annotation ;
            owl:onProperty linkml:annotations ],
        [ a owl:Restriction ;
            owl:allValuesFrom linkml:Example ;
            owl:onProperty linkml:examples ],
        [ a owl:Restriction ;
            owl:allValuesFrom linkml:AltDescription ;
            owl:onProperty linkml:alt_descriptions ],
        [ a owl:Restriction ;
            owl:maxQualifiedCardinality 1 ;
            owl:onClass linkml:Uriorcurie ;
            owl:onProperty bibo:status ],
        [ a owl:Restriction ;
            owl:maxQualifiedCardinality 1 ;
            owl:onClass linkml:Datetime ;
            owl:onProperty pav:lastUpdatedOn ],
        [ a owl:Restriction ;
            owl:allValuesFrom linkml:StructuredAlias ;
            owl:onProperty skosxl:altLabel ],
        [ a owl:Restriction ;
            owl:maxQualifiedCardinality 1 ;
            owl:onClass linkml:Boolean ;
            owl:onProperty sh:deactivated ],
        [ a owl:Restriction ;
            owl:allValuesFrom linkml:SubsetDefinition ;
            owl:onProperty OIO:inSubset ],
        [ a owl:Restriction ;
            owl:allValuesFrom linkml:String ;
            owl:onProperty skos:altLabel ],
        [ a owl:Restriction ;
            owl:allValuesFrom linkml:String ;
            owl:onProperty skos:editorialNote ],
        [ a owl:Restriction ;
            owl:maxQualifiedCardinality 1 ;
            owl:onClass linkml:Datetime ;
            owl:onProperty pav:createdOn ],
        [ a owl:Restriction ;
            owl:maxQualifiedCardinality 1 ;
            owl:onClass linkml:AnonymousClassExpression ;
            owl:onProperty sh:condition ],
        [ a owl:Restriction ;
            owl:allValuesFrom linkml:Uriorcurie ;
            owl:onProperty skos:narrowMatch ],
        [ a owl:Restriction ;
            owl:maxQualifiedCardinality 1 ;
            owl:onClass linkml:Integer ;
            owl:onProperty sh:order ],
        [ a owl:Restriction ;
            owl:maxQualifiedCardinality 1 ;
            owl:onClass linkml:AnonymousClassExpression ;
            owl:onProperty linkml:elseconditions ],
        [ a owl:Restriction ;
            owl:maxQualifiedCardinality 1 ;
            owl:onClass linkml:Boolean ;
            owl:onProperty linkml:open_world ],
        [ a owl:Restriction ;
            owl:allValuesFrom linkml:Uriorcurie ;
            owl:onProperty skos:closeMatch ],
        [ a owl:Restriction ;
            owl:allValuesFrom linkml:Uriorcurie ;
            owl:onProperty skos:exactMatch ],
        [ a owl:Restriction ;
            owl:allValuesFrom linkml:Extension ;
            owl:onProperty linkml:extensions ],
        [ a owl:Restriction ;
            owl:maxQualifiedCardinality 1 ;
            owl:onClass linkml:Uriorcurie ;
            owl:onProperty oslc:modifiedBy ],
        [ a owl:Restriction ;
            owl:allValuesFrom linkml:Uriorcurie ;
            owl:onProperty skos:relatedMatch ],
        [ a owl:Restriction ;
            owl:maxQualifiedCardinality 1 ;
            owl:onClass linkml:String ;
            owl:onProperty dcterms:title ],
        [ a owl:Restriction ;
            owl:maxQualifiedCardinality 1 ;
            owl:onClass linkml:Boolean ;
            owl:onProperty linkml:bidirectional ],
        [ a owl:Restriction ;
            owl:maxQualifiedCardinality 1 ;
            owl:onClass linkml:Uri ;
            owl:onProperty skos:inScheme ],
        [ a owl:Restriction ;
            owl:maxQualifiedCardinality 1 ;
            owl:onClass linkml:String ;
            owl:onProperty linkml:imported_from ],
        [ a owl:Restriction ;
            owl:maxQualifiedCardinality 1 ;
            owl:onClass linkml:AnonymousClassExpression ;
            owl:onProperty linkml:postconditions ],
        [ a owl:Restriction ;
            owl:maxQualifiedCardinality 1 ;
            owl:onClass linkml:String ;
            owl:onProperty linkml:deprecated ],
        [ a owl:Restriction ;
            owl:allValuesFrom linkml:Uriorcurie ;
            owl:onProperty skos:broadMatch ],
        [ a owl:Restriction ;
            owl:maxQualifiedCardinality 1 ;
            owl:onClass linkml:Uriorcurie ;
            owl:onProperty linkml:deprecated_element_has_exact_replacement ],
        linkml:Annotatable,
        linkml:ClassLevelRule,
        linkml:CommonMetadata,
        linkml:Extensible ;
    skos:altLabel "if rule" ;
    skos:closeMatch swrl:Imp,
        sh:TripleRule ;
    skos:definition "A rule that applies to instances of a class" .

<https://w3id.org/linkml/PresenceEnum#ABSENT> a owl:Class,
        linkml:PresenceEnum ;
    rdfs:label "ABSENT" .

<https://w3id.org/linkml/PresenceEnum#PRESENT> a owl:Class,
        linkml:PresenceEnum ;
    rdfs:label "PRESENT" .

<https://w3id.org/linkml/PresenceEnum#UNCOMMITTED> a owl:Class,
        linkml:PresenceEnum ;
    rdfs:label "UNCOMMITTED" .

<https://w3id.org/linkml/PvFormulaOptions#CODE> a owl:Class,
        linkml:PvFormulaOptions ;
    rdfs:label "CODE" .

<https://w3id.org/linkml/PvFormulaOptions#CURIE> a owl:Class,
        linkml:PvFormulaOptions ;
    rdfs:label "CURIE" .

<https://w3id.org/linkml/PvFormulaOptions#FHIR_CODING> a owl:Class,
        linkml:PvFormulaOptions ;
    rdfs:label "FHIR_CODING" .

<https://w3id.org/linkml/PvFormulaOptions#URI> a owl:Class,
        linkml:PvFormulaOptions ;
    rdfs:label "URI" .

<https://w3id.org/linkml/RelationalRoleEnum#NODE> a owl:Class,
        linkml:RelationalRoleEnum ;
    rdfs:label "NODE" .

<https://w3id.org/linkml/RelationalRoleEnum#OTHER_ROLE> a owl:Class,
        linkml:RelationalRoleEnum ;
    rdfs:label "OTHER_ROLE" .

linkml:TypeExpression a owl:Class,
        linkml:ClassDefinition ;
    rdfs:label "type_expression" ;
    rdfs:subClassOf [ a owl:Restriction ;
            owl:allValuesFrom linkml:AnonymousTypeExpression ;
            owl:onProperty linkml:any_of ],
        [ a owl:Restriction ;
            owl:allValuesFrom linkml:String ;
            owl:onProperty linkml:equals_string_in ],
        [ a owl:Restriction ;
            owl:maxQualifiedCardinality 1 ;
            owl:onClass linkml:Integer ;
            owl:onProperty linkml:equals_number ],
        [ a owl:Restriction ;
            owl:maxQualifiedCardinality 1 ;
            owl:onClass linkml:String ;
            owl:onProperty linkml:implicit_prefix ],
        [ a owl:Restriction ;
            owl:maxQualifiedCardinality 1 ;
            owl:onClass linkml:String ;
            owl:onProperty linkml:equals_string ],
        [ a owl:Restriction ;
            owl:allValuesFrom linkml:AnonymousTypeExpression ;
            owl:onProperty linkml:none_of ],
        [ a owl:Restriction ;
            owl:maxQualifiedCardinality 1 ;
            owl:onClass linkml:PatternExpression ;
            owl:onProperty linkml:structured_pattern ],
        [ a owl:Restriction ;
            owl:maxQualifiedCardinality 1 ;
            owl:onClass linkml:Integer ;
            owl:onProperty linkml:minimum_value ],
        [ a owl:Restriction ;
            owl:allValuesFrom linkml:AnonymousTypeExpression ;
            owl:onProperty linkml:all_of ],
        [ a owl:Restriction ;
            owl:allValuesFrom linkml:AnonymousTypeExpression ;
            owl:onProperty linkml:exactly_one_of ],
        [ a owl:Restriction ;
            owl:maxQualifiedCardinality 1 ;
            owl:onClass linkml:Integer ;
            owl:onProperty linkml:maximum_value ],
        [ a owl:Restriction ;
            owl:maxQualifiedCardinality 1 ;
            owl:onClass linkml:UnitOfMeasure ;
            owl:onProperty qudt:unit ],
        [ a owl:Restriction ;
            owl:maxQualifiedCardinality 1 ;
            owl:onClass linkml:String ;
            owl:onProperty linkml:pattern ],
        linkml:Expression,
        linkml:mixin ;
    skos:definition "An abstract class grouping named types and anonymous type expressions" .

linkml:children_are_mutually_disjoint a owl:ObjectProperty,
        linkml:SlotDefinition ;
    rdfs:label "children_are_mutually_disjoint" ;
    rdfs:domain linkml:Definition ;
    rdfs:range linkml:Boolean ;
    skos:definition "If true then all direct is_a children are mutually disjoint and share no instances in common" .

linkml:disjoint_with a owl:ObjectProperty,
        linkml:SlotDefinition ;
    rdfs:label "disjoint_with" ;
    rdfs:domain linkml:Definition ;
    rdfs:range linkml:Definition ;
    skos:definition "Two classes are disjoint if they have no instances in common, two slots are disjoint if they can never hold between the same two instances" .

linkml:slot_names_unique a owl:ObjectProperty,
        linkml:SlotDefinition ;
    rdfs:label "slot_names_unique" ;
    rdfs:domain linkml:Definition ;
    rdfs:range linkml:Boolean ;
    skos:definition "if true then induced/mangled slot names are not created for class_usage and attributes" .

linkml:slots a owl:ObjectProperty,
        linkml:SlotDefinition .

linkml:source_ontology a owl:ObjectProperty,
        linkml:SlotDefinition ;
    rdfs:label "source_ontology" ;
    rdfs:range linkml:Uriorcurie ;
    skos:altLabel "terminology",
        "vocabulary" ;
    skos:definition "An ontology or vocabulary or terminology that is used in a query to obtain a set of permissible values" ;
    skos:note "examples include schema.org, wikidata, or an OBO ontology",
        "for obo ontologies we recommend CURIEs of the form obo:cl, obo:envo, etc" .

linkml:transitive_form_of a owl:ObjectProperty,
        linkml:SlotDefinition ;
    rdfs:label "transitive_form_of" ;
    rdfs:range linkml:SlotDefinition ;
    skos:definition "If s transitive_form_of d, then (1) s holds whenever d holds (2) s is transitive (3) d holds whenever s holds and there are no intermediates, and s is not reflexive" ;
    skos:note "Example: ancestor_of is the transitive_form_of parent_of" .

linkml:unique_key_slots a owl:ObjectProperty,
        linkml:SlotDefinition ;
    rdfs:label "unique_key_slots" ;
    rdfs:domain linkml:UniqueKey ;
    rdfs:range linkml:SlotDefinition ;
    skos:definition "list of slot names that form a key. The tuple formed from the values of all these slots should be unique." .

dcterms:subject a owl:ObjectProperty,
        linkml:SlotDefinition ;
    rdfs:label "categories" ;
    rdfs:range linkml:Uriorcurie ;
    skos:definition "Controlled terms used to categorize an element." ;
    skos:exactMatch dcterms:subject ;
    skos:note "if you wish to use uncontrolled terms or terms that lack identifiers then use the keywords element" .

rdfs:label a owl:ObjectProperty,
        linkml:SlotDefinition .

linkml:Anything a owl:Class,
        linkml:ClassDefinition ;
    rdfs:label "Anything" ;
    skos:exactMatch linkml:Any .

linkml:all_members a owl:ObjectProperty,
        linkml:SlotDefinition ;
    rdfs:label "all_members" ;
    rdfs:range linkml:AnonymousSlotExpression ;
    rdfs:subPropertyOf linkml:list_value_specification_constant ;
    skos:definition "the value of the slot is multivalued with all members satisfying the condition" .

linkml:apply_to a owl:ObjectProperty,
        linkml:SlotDefinition ;
    rdfs:label "apply_to" ;
    rdfs:domain linkml:Definition ;
    rdfs:range linkml:Definition ;
    skos:definition "Used to extend class or slot definitions. For example, if we have a core schema where a gene has two slots for identifier and symbol, and we have a specialized schema for my_organism where we wish to add a slot systematic_name, we can avoid subclassing by defining a class gene_my_organism, adding the slot to this class, and then adding an apply_to pointing to the gene class. The new slot will be 'injected into' the gene class." .

linkml:code_set a owl:ObjectProperty,
        linkml:SlotDefinition ;
    rdfs:label "code_set" ;
    rdfs:domain linkml:EnumExpression ;
    rdfs:range linkml:Uriorcurie ;
    skos:definition "the identifier of an enumeration code set." .

linkml:code_set_tag a owl:ObjectProperty,
        linkml:SlotDefinition ;
    rdfs:label "code_set_tag" ;
    rdfs:domain linkml:EnumExpression ;
    rdfs:range linkml:String ;
    skos:definition "the version tag of the enumeration code set" ;
    skos:note "enum_expression cannot have both a code_set_tag and a code_set_version" .

linkml:code_set_version a owl:ObjectProperty,
        linkml:SlotDefinition ;
    rdfs:label "code_set_version" ;
    rdfs:domain linkml:EnumExpression ;
    rdfs:range linkml:String ;
    skos:definition "the version identifier of the enumeration code set" ;
    skos:note "we assume that version identifiers lexically sort in temporal order. Recommend semver when possible" .

linkml:concepts a owl:ObjectProperty,
        linkml:SlotDefinition ;
    rdfs:label "concepts" ;
    rdfs:domain linkml:EnumExpression ;
    rdfs:range linkml:Uriorcurie ;
    skos:definition "A list of identifiers that are used to construct a set of permissible values" .

linkml:enum_range a owl:ObjectProperty,
        linkml:SlotDefinition ;
    rdfs:label "enum_range" ;
    rdfs:range linkml:EnumExpression ;
    skos:definition "An inlined enumeration" .

linkml:equals_expression a owl:ObjectProperty,
        linkml:SlotDefinition ;
    rdfs:label "equals_expression" ;
    rdfs:range linkml:String ;
    rdfs:seeAlso "https://linkml.io/linkml/developers/inference.html",
        "https://linkml.io/linkml/schemas/advanced.html#equals-expression" ;
    rdfs:subPropertyOf linkml:list_value_specification_constant ;
    skos:definition "the value of the slot must equal the value of the evaluated expression" ;
    skos:note "for example, a 'length' slot may have an equals_expression with value '(end-start)+1'" .

linkml:has_member a owl:ObjectProperty,
        linkml:SlotDefinition ;
    rdfs:label "has_member" ;
    rdfs:range linkml:AnonymousSlotExpression ;
    rdfs:subPropertyOf linkml:list_value_specification_constant ;
    skos:definition "the value of the slot is multivalued with at least one member satisfying the condition" .

linkml:include a owl:ObjectProperty,
        linkml:SlotDefinition ;
    rdfs:label "include" ;
    rdfs:domain linkml:EnumExpression ;
    rdfs:range linkml:AnonymousEnumExpression ;
    skos:definition "An enum expression that yields a list of permissible values that are to be included, after subtracting the minus set" .

linkml:inherits a owl:ObjectProperty,
        linkml:SlotDefinition ;
    rdfs:label "inherits" ;
    rdfs:domain linkml:EnumExpression ;
    rdfs:range linkml:EnumDefinition ;
    skos:definition "An enum definition that is used as the basis to create a new enum" ;
    skos:note "All permissible values for all inherited enums are copied to form the initial seed set" .

linkml:inlined a owl:ObjectProperty,
        linkml:SlotDefinition ;
    rdfs:label "inlined" ;
    rdfs:domain linkml:SlotDefinition ;
    rdfs:range linkml:Boolean ;
    rdfs:seeAlso "https://w3id.org/linkml/docs/specification/06mapping/#collection-forms" ;
    skos:definition "True means that keyed or identified slot appears in an outer structure by value.  False means that only the key or identifier for the slot appears within the domain, referencing a structure that appears elsewhere." ;
    skos:note "classes without keys or identifiers are necessarily inlined as lists",
        "only applicable in tree-like serializations, e.g json, yaml" .

linkml:inlined_as_list a owl:ObjectProperty,
        linkml:SlotDefinition ;
    rdfs:label "inlined_as_list" ;
    rdfs:domain linkml:SlotDefinition ;
    rdfs:range linkml:Boolean ;
    rdfs:seeAlso "https://w3id.org/linkml/docs/specification/06mapping/#collection-forms" ;
    skos:definition "True means that an inlined slot is represented as a list of range instances.  False means that an inlined slot is represented as a dictionary, whose key is the slot key or identifier and whose value is the range instance." ;
    skos:note """A keyed or identified class with one additional slot can be input in a third form, a dictionary whose key
is the key or identifier and whose value is the one additional element.  This form is still stored according
to the inlined_as_list setting.""",
        """The default loader will accept either list or dictionary form as input.  This parameter controls internal
representation and output.""" .

linkml:matches a owl:ObjectProperty,
        linkml:SlotDefinition ;
    rdfs:label "matches" ;
    rdfs:domain linkml:EnumExpression ;
    rdfs:range linkml:MatchQuery ;
    skos:definition "Specifies a match query that is used to calculate the list of permissible values" .

linkml:maximum_cardinality a owl:ObjectProperty,
        linkml:SlotDefinition ;
    rdfs:label "maximum_cardinality" ;
    rdfs:range linkml:Integer ;
    rdfs:subPropertyOf linkml:list_value_specification_constant ;
    skos:definition "the maximum number of entries for a multivalued slot" .

linkml:minimum_cardinality a owl:ObjectProperty,
        linkml:SlotDefinition ;
    rdfs:label "minimum_cardinality" ;
    rdfs:range linkml:Integer ;
    rdfs:subPropertyOf linkml:list_value_specification_constant ;
    skos:definition "the minimum number of entries for a multivalued slot" .

linkml:minus a owl:ObjectProperty,
        linkml:SlotDefinition ;
    rdfs:label "minus" ;
    rdfs:domain linkml:EnumExpression ;
    rdfs:range linkml:AnonymousEnumExpression ;
    skos:definition "An enum expression that yields a list of permissible values that are to be subtracted from the enum" .

linkml:permissible_values a owl:ObjectProperty,
        linkml:SlotDefinition ;
    rdfs:label "permissible_values" ;
    rdfs:domain linkml:EnumExpression ;
    rdfs:range linkml:PermissibleValue ;
    skos:altLabel "coded values" ;
    skos:definition "A list of possible values for a slot range" .

linkml:pv_formula a owl:ObjectProperty,
        linkml:SlotDefinition ;
    rdfs:label "pv_formula" ;
    rdfs:domain linkml:EnumExpression ;
    rdfs:range linkml:PvFormulaOptions ;
    skos:definition "Defines the specific formula to be used to generate the permissible values." ;
    skos:note "code_set must be supplied for this to be valid",
        "you cannot have BOTH the permissible_values and permissible_value_formula tag" .

linkml:range a owl:ObjectProperty,
        linkml:SlotDefinition ;
    rdfs:label "range" ;
    rdfs:domain linkml:SlotDefinition ;
    rdfs:range linkml:Element ;
    skos:altLabel "value domain" ;
    skos:definition """defines the type of the object of the slot.  Given the following slot definition
  S1:
    domain: C1
    range:  C2
the declaration
  X:
    S1: Y

implicitly asserts Y is an instance of C2
""" ;
    skos:note "range is underspecified, as not all elements can appear as the range of a slot." .

linkml:reachable_from a owl:ObjectProperty,
        linkml:SlotDefinition ;
    rdfs:label "reachable_from" ;
    rdfs:domain linkml:EnumExpression ;
    rdfs:range linkml:ReachabilityQuery ;
    skos:definition "Specifies a query for obtaining a list of permissible values based on graph reachability" .

linkml:recommended a owl:ObjectProperty,
        linkml:SlotDefinition ;
    rdfs:label "recommended" ;
    rdfs:domain linkml:SlotDefinition ;
    rdfs:range linkml:Boolean ;
    rdfs:seeAlso "https://github.com/linkml/linkml/issues/177" ;
    skos:definition "true means that the slot should be present in instances of the class definition, but this is not required" ;
    skos:note "If a slot is recommended, and it is not populated, applications must not treat this as an error. Applications may use this to inform the user of missing data",
        "This is to be used where not all data is expected to conform to having a required field" .

linkml:required a owl:ObjectProperty,
        linkml:SlotDefinition ;
    rdfs:label "required" ;
    rdfs:domain linkml:SlotDefinition ;
    rdfs:range linkml:Boolean ;
    skos:definition "true means that the slot must be present in instances of the class definition" .

linkml:slot_conditions a owl:ObjectProperty,
        linkml:SlotDefinition ;
    rdfs:label "slot_conditions" ;
    rdfs:domain linkml:ClassExpression ;
    rdfs:range linkml:SlotDefinition ;
    skos:definition "expresses constraints on a group of slots for a class expression" .

linkml:union_of a owl:ObjectProperty,
        linkml:SlotDefinition ;
    rdfs:label "union_of" ;
    rdfs:domain linkml:Element ;
    rdfs:range linkml:Element ;
    skos:definition "indicates that the domain element consists exactly of the members of the element in the range." ;
    skos:editorialNote "this only applies in the OWL generation" .

linkml:value_presence a owl:ObjectProperty,
        linkml:SlotDefinition ;
    rdfs:label "value_presence" ;
    rdfs:domain linkml:SlotDefinition ;
    rdfs:range linkml:PresenceEnum ;
    rdfs:subPropertyOf linkml:list_value_specification_constant ;
    skos:definition "if true then a value must be present (for lists there must be at least one value). If false then a value must be absent (for lists, must be empty)" ;
    skos:note "if set to true this has the same effect as required=true. In contrast, required=false allows a value to be present" .

rdf:predicate a owl:Class,
        owl:ObjectProperty,
        linkml:RelationalRoleEnum,
        linkml:SlotDefinition ;
    rdfs:label "PREDICATE",
        "predicate" ;
    rdfs:domain linkml:StructuredAlias ;
    rdfs:range linkml:AliasPredicateEnum ;
    skos:definition "The relationship between an element and its alias." ;
    skos:exactMatch rdf:predicate .

linkml:ClassExpression a owl:Class,
        linkml:ClassDefinition ;
    rdfs:label "class_expression" ;
    rdfs:subClassOf [ a owl:Restriction ;
            owl:allValuesFrom linkml:AnonymousClassExpression ;
            owl:onProperty linkml:any_of ],
        [ a owl:Restriction ;
            owl:allValuesFrom linkml:AnonymousClassExpression ;
            owl:onProperty linkml:none_of ],
        [ a owl:Restriction ;
            owl:allValuesFrom linkml:SlotDefinition ;
            owl:onProperty linkml:slot_conditions ],
        [ a owl:Restriction ;
            owl:allValuesFrom linkml:AnonymousClassExpression ;
            owl:onProperty linkml:all_of ],
        [ a owl:Restriction ;
            owl:allValuesFrom linkml:AnonymousClassExpression ;
            owl:onProperty linkml:exactly_one_of ],
        linkml:mixin ;
    skos:definition "A boolean expression that can be used to dynamically determine membership of a class" .

linkml:ImportExpression a owl:Class,
        linkml:ClassDefinition ;
    rdfs:label "import_expression" ;
    rdfs:subClassOf [ a owl:Restriction ;
            owl:allValuesFrom linkml:Uriorcurie ;
            owl:onProperty skos:exactMatch ],
        [ a owl:Restriction ;
            owl:maxQualifiedCardinality 1 ;
            owl:onClass linkml:Datetime ;
            owl:onProperty pav:createdOn ],
        [ a owl:Restriction ;
            owl:allValuesFrom linkml:StructuredAlias ;
            owl:onProperty skosxl:altLabel ],
        [ a owl:Restriction ;
            owl:allValuesFrom linkml:String ;
            owl:onProperty linkml:todos ],
        [ a owl:Restriction ;
            owl:maxQualifiedCardinality 1 ;
            owl:onClass linkml:Uriorcurie ;
            owl:onProperty linkml:deprecated_element_has_exact_replacement ],
        [ a owl:Restriction ;
            owl:maxQualifiedCardinality 1 ;
            owl:onClass linkml:Uriorcurie ;
            owl:onProperty oslc:modifiedBy ],
        [ a owl:Restriction ;
            owl:maxQualifiedCardinality 1 ;
            owl:onClass linkml:Uri ;
            owl:onProperty skos:inScheme ],
        [ a owl:Restriction ;
            owl:maxQualifiedCardinality 1 ;
            owl:onClass linkml:Ncname ;
            owl:onProperty linkml:import_as ],
        [ a owl:Restriction ;
            owl:maxQualifiedCardinality 1 ;
            owl:onClass linkml:Datetime ;
            owl:onProperty pav:lastUpdatedOn ],
        [ a owl:Restriction ;
            owl:allValuesFrom linkml:String ;
            owl:onProperty skos:note ],
        [ a owl:Restriction ;
            owl:maxQualifiedCardinality 1 ;
            owl:onClass linkml:String ;
            owl:onProperty linkml:imported_from ],
        [ a owl:Restriction ;
            owl:allValuesFrom linkml:Extension ;
            owl:onProperty linkml:extensions ],
        [ a owl:Restriction ;
            owl:maxQualifiedCardinality 1 ;
            owl:onClass linkml:String ;
            owl:onProperty skos:definition ],
        [ a owl:Restriction ;
            owl:allValuesFrom linkml:Uriorcurie ;
            owl:onProperty rdfs:seeAlso ],
        [ a owl:Restriction ;
            owl:maxQualifiedCardinality 1 ;
            owl:onClass linkml:Uriorcurie ;
            owl:onProperty dcterms:source ],
        [ a owl:Restriction ;
            owl:allValuesFrom linkml:Example ;
            owl:onProperty linkml:examples ],
        [ a owl:Restriction ;
            owl:maxQualifiedCardinality 1 ;
            owl:onClass linkml:String ;
            owl:onProperty schema:inLanguage ],
        [ a owl:Restriction ;
            owl:maxQualifiedCardinality 1 ;
            owl:onClass linkml:String ;
            owl:onProperty linkml:deprecated ],
        [ a owl:Restriction ;
            owl:allValuesFrom linkml:SubsetDefinition ;
            owl:onProperty OIO:inSubset ],
        [ a owl:Restriction ;
            owl:allValuesFrom linkml:Setting ;
            owl:onProperty linkml:import_map ],
        [ a owl:Restriction ;
            owl:allValuesFrom linkml:Uriorcurie ;
            owl:onProperty skos:relatedMatch ],
        [ a owl:Restriction ;
            owl:allValuesFrom linkml:String ;
            owl:onProperty skos:altLabel ],
        [ a owl:Restriction ;
            owl:maxQualifiedCardinality 1 ;
            owl:onClass linkml:Uriorcurie ;
            owl:onProperty linkml:deprecated_element_has_possible_replacement ],
        [ a owl:Restriction ;
            owl:allValuesFrom linkml:Annotation ;
            owl:onProperty linkml:annotations ],
        [ a owl:Restriction ;
            owl:maxQualifiedCardinality 1 ;
            owl:onClass linkml:Uriorcurie ;
            owl:onProperty bibo:status ],
        [ a owl:Restriction ;
            owl:maxQualifiedCardinality 1 ;
            owl:onClass linkml:Uriorcurie ;
            owl:onProperty pav:createdBy ],
        [ a owl:Restriction ;
            owl:allValuesFrom linkml:Uriorcurie ;
            owl:onProperty skos:broadMatch ],
        [ a owl:Restriction ;
            owl:maxQualifiedCardinality 1 ;
            owl:onClass linkml:Integer ;
            owl:onProperty sh:order ],
        [ a owl:Restriction ;
            owl:allValuesFrom linkml:AltDescription ;
            owl:onProperty linkml:alt_descriptions ],
        [ a owl:Restriction ;
            owl:allValuesFrom linkml:Uriorcurie ;
            owl:onProperty skos:narrowMatch ],
        [ a owl:Restriction ;
            owl:onClass linkml:Uriorcurie ;
            owl:onProperty linkml:import_from ;
            owl:qualifiedCardinality 1 ],
        [ a owl:Restriction ;
            owl:allValuesFrom linkml:Uriorcurie ;
            owl:onProperty skos:mappingRelation ],
        [ a owl:Restriction ;
            owl:maxQualifiedCardinality 1 ;
            owl:onClass linkml:String ;
            owl:onProperty dcterms:title ],
        [ a owl:Restriction ;
            owl:allValuesFrom linkml:Uriorcurie ;
            owl:onProperty skos:closeMatch ],
        [ a owl:Restriction ;
            owl:allValuesFrom linkml:String ;
            owl:onProperty skos:editorialNote ],
        linkml:Annotatable,
        linkml:CommonMetadata,
        linkml:Extensible ;
    skos:definition "an expression describing an import" .

linkml:LocalName a owl:Class,
        linkml:ClassDefinition ;
    rdfs:label "local_name" ;
    rdfs:subClassOf [ a owl:Restriction ;
            owl:onClass linkml:Ncname ;
            owl:onProperty linkml:local_name_source ;
            owl:qualifiedCardinality 1 ],
        [ a owl:Restriction ;
            owl:onClass linkml:String ;
            owl:onProperty skos:altLabel ;
            owl:qualifiedCardinality 1 ] ;
    skos:definition "an attributed label" .

linkml:SlotExpression a owl:Class,
        linkml:ClassDefinition ;
    rdfs:label "slot_expression" ;
    rdfs:subClassOf [ a owl:Restriction ;
            owl:maxQualifiedCardinality 1 ;
            owl:onClass linkml:Integer ;
            owl:onProperty linkml:minimum_value ],
        [ a owl:Restriction ;
            owl:maxQualifiedCardinality 1 ;
            owl:onClass linkml:Element ;
            owl:onProperty linkml:range ],
        [ a owl:Restriction ;
            owl:maxQualifiedCardinality 1 ;
            owl:onClass linkml:Integer ;
            owl:onProperty linkml:maximum_cardinality ],
        [ a owl:Restriction ;
            owl:maxQualifiedCardinality 1 ;
            owl:onClass linkml:PatternExpression ;
            owl:onProperty linkml:structured_pattern ],
        [ a owl:Restriction ;
            owl:allValuesFrom linkml:AnonymousSlotExpression ;
            owl:onProperty linkml:none_of ],
        [ a owl:Restriction ;
            owl:maxQualifiedCardinality 1 ;
            owl:onClass linkml:Boolean ;
            owl:onProperty linkml:required ],
        [ a owl:Restriction ;
            owl:maxQualifiedCardinality 1 ;
            owl:onClass linkml:UnitOfMeasure ;
            owl:onProperty qudt:unit ],
        [ a owl:Restriction ;
            owl:maxQualifiedCardinality 1 ;
            owl:onClass linkml:AnonymousSlotExpression ;
            owl:onProperty linkml:all_members ],
        [ a owl:Restriction ;
            owl:allValuesFrom linkml:AnonymousSlotExpression ;
            owl:onProperty linkml:exactly_one_of ],
        [ a owl:Restriction ;
            owl:allValuesFrom linkml:AnonymousSlotExpression ;
            owl:onProperty linkml:any_of ],
        [ a owl:Restriction ;
            owl:maxQualifiedCardinality 1 ;
            owl:onClass linkml:Integer ;
            owl:onProperty linkml:minimum_cardinality ],
        [ a owl:Restriction ;
            owl:maxQualifiedCardinality 1 ;
            owl:onClass linkml:PresenceEnum ;
            owl:onProperty linkml:value_presence ],
        [ a owl:Restriction ;
            owl:allValuesFrom linkml:String ;
            owl:onProperty linkml:equals_string_in ],
        [ a owl:Restriction ;
            owl:maxQualifiedCardinality 1 ;
            owl:onClass linkml:Boolean ;
            owl:onProperty linkml:inlined_as_list ],
        [ a owl:Restriction ;
            owl:maxQualifiedCardinality 1 ;
            owl:onClass linkml:AnonymousSlotExpression ;
            owl:onProperty linkml:has_member ],
        [ a owl:Restriction ;
            owl:maxQualifiedCardinality 1 ;
            owl:onClass linkml:Integer ;
            owl:onProperty linkml:equals_number ],
        [ a owl:Restriction ;
            owl:maxQualifiedCardinality 1 ;
            owl:onClass linkml:String ;
            owl:onProperty linkml:equals_string ],
        [ a owl:Restriction ;
            owl:allValuesFrom linkml:AnonymousSlotExpression ;
            owl:onProperty linkml:all_of ],
        [ a owl:Restriction ;
            owl:maxQualifiedCardinality 1 ;
            owl:onClass linkml:Boolean ;
            owl:onProperty linkml:recommended ],
        [ a owl:Restriction ;
            owl:maxQualifiedCardinality 1 ;
            owl:onClass linkml:String ;
            owl:onProperty linkml:implicit_prefix ],
        [ a owl:Restriction ;
            owl:maxQualifiedCardinality 1 ;
            owl:onClass linkml:Boolean ;
            owl:onProperty linkml:inlined ],
        [ a owl:Restriction ;
            owl:maxQualifiedCardinality 1 ;
            owl:onClass linkml:String ;
            owl:onProperty linkml:equals_expression ],
        [ a owl:Restriction ;
            owl:maxQualifiedCardinality 1 ;
            owl:onClass linkml:AnonymousClassExpression ;
            owl:onProperty linkml:range_expression ],
        [ a owl:Restriction ;
            owl:maxQualifiedCardinality 1 ;
            owl:onClass linkml:EnumExpression ;
            owl:onProperty linkml:enum_range ],
        [ a owl:Restriction ;
            owl:maxQualifiedCardinality 1 ;
            owl:onClass linkml:String ;
            owl:onProperty linkml:pattern ],
        [ a owl:Restriction ;
            owl:maxQualifiedCardinality 1 ;
            owl:onClass linkml:Integer ;
            owl:onProperty linkml:maximum_value ],
        linkml:Expression,
        linkml:mixin ;
    skos:definition "an expression that constrains the range of values a slot can take" .

linkml:boolean_slot a owl:ObjectProperty,
        linkml:SlotDefinition ;
    rdfs:label "boolean_slot" ;
    rdfs:range linkml:Expression ;
    skos:definition "A grouping of slots that expression a boolean operator over a list of operands" .

linkml:mixins a owl:ObjectProperty,
        linkml:SlotDefinition ;
    rdfs:label "mixins" ;
    rdfs:domain linkml:Definition ;
    rdfs:range linkml:Definition ;
    rdfs:seeAlso "https://en.wikipedia.org/wiki/Mixin" ;
    skos:altLabel "traits" ;
    skos:definition "A collection of secondary parent classes or slots from which inheritable metaslots are propagated from." ;
    skos:note "mixins act in the same way as parents (is_a). They allow a model to have a primary strict hierachy, while keeping the benefits of multiple inheritance" .

linkml:range_expression a owl:ObjectProperty,
        linkml:SlotDefinition ;
    rdfs:label "range_expression" ;
    rdfs:domain linkml:SlotExpression ;
    rdfs:range linkml:AnonymousClassExpression ;
    skos:definition "A range that is described as a boolean expression combining existing ranges" ;
    skos:note "one use for this is being able to describe a range using any_of expressions, for example to combine two enums" .

linkml:Prefix a owl:Class,
        linkml:ClassDefinition ;
    rdfs:label "prefix" ;
    rdfs:subClassOf [ a owl:Restriction ;
            owl:onClass linkml:Ncname ;
            owl:onProperty sh:prefix ;
            owl:qualifiedCardinality 1 ],
        [ a owl:Restriction ;
            owl:onClass linkml:Uri ;
            owl:onProperty sh:namespace ;
            owl:qualifiedCardinality 1 ] ;
    skos:definition "prefix URI tuple" .

linkml:UniqueKey a owl:Class,
        linkml:ClassDefinition ;
    rdfs:label "unique_key" ;
    rdfs:subClassOf [ a owl:Restriction ;
            owl:allValuesFrom linkml:StructuredAlias ;
            owl:onProperty skosxl:altLabel ],
        [ a owl:Restriction ;
            owl:maxQualifiedCardinality 1 ;
            owl:onClass linkml:String ;
            owl:onProperty dcterms:title ],
        [ a owl:Restriction ;
            owl:allValuesFrom linkml:Example ;
            owl:onProperty linkml:examples ],
        [ a owl:Restriction ;
            owl:allValuesFrom linkml:Uriorcurie ;
            owl:onProperty skos:exactMatch ],
        [ a owl:Class ;
            owl:intersectionOf ( [ a owl:Restriction ;
                        owl:allValuesFrom linkml:SlotDefinition ;
                        owl:onProperty linkml:unique_key_slots ] [ a owl:Restriction ;
                        owl:onProperty linkml:unique_key_slots ;
                        owl:someValuesFrom linkml:SlotDefinition ] ) ],
        [ a owl:Restriction ;
            owl:maxQualifiedCardinality 1 ;
            owl:onClass linkml:Uriorcurie ;
            owl:onProperty dcterms:source ],
        [ a owl:Restriction ;
            owl:allValuesFrom linkml:String ;
            owl:onProperty linkml:todos ],
        [ a owl:Restriction ;
            owl:maxQualifiedCardinality 1 ;
            owl:onClass linkml:Boolean ;
            owl:onProperty linkml:consider_nulls_inequal ],
        [ a owl:Restriction ;
            owl:maxQualifiedCardinality 1 ;
            owl:onClass linkml:Uriorcurie ;
            owl:onProperty bibo:status ],
        [ a owl:Restriction ;
            owl:allValuesFrom linkml:Uriorcurie ;
            owl:onProperty skos:narrowMatch ],
        [ a owl:Restriction ;
            owl:maxQualifiedCardinality 1 ;
            owl:onClass linkml:Integer ;
            owl:onProperty sh:order ],
        [ a owl:Restriction ;
            owl:maxQualifiedCardinality 1 ;
            owl:onClass linkml:Uri ;
            owl:onProperty skos:inScheme ],
        [ a owl:Restriction ;
            owl:allValuesFrom linkml:Uriorcurie ;
            owl:onProperty skos:relatedMatch ],
        [ a owl:Restriction ;
            owl:maxQualifiedCardinality 1 ;
            owl:onClass linkml:String ;
            owl:onProperty skos:definition ],
        [ a owl:Restriction ;
            owl:allValuesFrom linkml:AltDescription ;
            owl:onProperty linkml:alt_descriptions ],
        [ a owl:Restriction ;
            owl:maxQualifiedCardinality 1 ;
            owl:onClass linkml:Datetime ;
            owl:onProperty pav:lastUpdatedOn ],
        [ a owl:Restriction ;
            owl:onClass linkml:String ;
            owl:onProperty linkml:unique_key_name ;
            owl:qualifiedCardinality 1 ],
        [ a owl:Restriction ;
            owl:maxQualifiedCardinality 1 ;
            owl:onClass linkml:Uriorcurie ;
            owl:onProperty linkml:deprecated_element_has_exact_replacement ],
        [ a owl:Restriction ;
            owl:maxQualifiedCardinality 1 ;
            owl:onClass linkml:String ;
            owl:onProperty linkml:imported_from ],
        [ a owl:Restriction ;
            owl:allValuesFrom linkml:SubsetDefinition ;
            owl:onProperty OIO:inSubset ],
        [ a owl:Restriction ;
            owl:maxQualifiedCardinality 1 ;
            owl:onClass linkml:Uriorcurie ;
            owl:onProperty pav:createdBy ],
        [ a owl:Restriction ;
            owl:allValuesFrom linkml:String ;
            owl:onProperty skos:editorialNote ],
        [ a owl:Restriction ;
            owl:allValuesFrom linkml:Uriorcurie ;
            owl:onProperty skos:closeMatch ],
        [ a owl:Restriction ;
            owl:maxQualifiedCardinality 1 ;
            owl:onClass linkml:Datetime ;
            owl:onProperty pav:createdOn ],
        [ a owl:Restriction ;
            owl:maxQualifiedCardinality 1 ;
            owl:onClass linkml:Uriorcurie ;
            owl:onProperty oslc:modifiedBy ],
        [ a owl:Restriction ;
            owl:maxQualifiedCardinality 1 ;
            owl:onClass linkml:Uriorcurie ;
            owl:onProperty linkml:deprecated_element_has_possible_replacement ],
        [ a owl:Restriction ;
            owl:allValuesFrom linkml:Uriorcurie ;
            owl:onProperty rdfs:seeAlso ],
        [ a owl:Restriction ;
            owl:allValuesFrom linkml:String ;
            owl:onProperty skos:altLabel ],
        [ a owl:Restriction ;
            owl:maxQualifiedCardinality 1 ;
            owl:onClass linkml:String ;
            owl:onProperty linkml:deprecated ],
        [ a owl:Restriction ;
            owl:allValuesFrom linkml:String ;
            owl:onProperty skos:note ],
        [ a owl:Restriction ;
            owl:maxQualifiedCardinality 1 ;
            owl:onClass linkml:String ;
            owl:onProperty schema:inLanguage ],
        [ a owl:Restriction ;
            owl:allValuesFrom linkml:Uriorcurie ;
            owl:onProperty skos:broadMatch ],
        [ a owl:Restriction ;
            owl:allValuesFrom linkml:Uriorcurie ;
            owl:onProperty skos:mappingRelation ],
        [ a owl:Restriction ;
            owl:allValuesFrom linkml:Annotation ;
            owl:onProperty linkml:annotations ],
        [ a owl:Restriction ;
            owl:allValuesFrom linkml:Extension ;
            owl:onProperty linkml:extensions ],
        linkml:Annotatable,
        linkml:CommonMetadata,
        linkml:Extensible ;
    skos:definition "a collection of slots whose values uniquely identify an instance of a class" .

linkml:is_a a owl:ObjectProperty,
        linkml:SlotDefinition ;
    rdfs:label "is_a" ;
    rdfs:domain linkml:Definition ;
    rdfs:range linkml:Definition ;
    skos:definition "A primary parent class or slot from which inheritable metaslots are propagated from. While multiple inheritance is not allowed, mixins can be provided effectively providing the same thing. The semantics are the same when translated to formalisms that allow MI (e.g. RDFS/OWL). When translating to a SI framework (e.g. java classes, python classes) then is a is used. When translating a framework without polymorphism (e.g. json-schema, solr document schema) then is a and mixins are recursively unfolded" .

linkml:AliasPredicateEnum a owl:Class,
        linkml:EnumDefinition ;
    rdfs:label "alias_predicate_enum" ;
    owl:unionOf ( skos:exactMatch skos:relatedMatch skos:broaderMatch skos:narrowerMatch ) ;
    linkml:permissible_values skos:broaderMatch,
        skos:exactMatch,
        skos:narrowerMatch,
        skos:relatedMatch .

linkml:MatchQuery a owl:Class,
        linkml:ClassDefinition ;
    rdfs:label "match_query" ;
    rdfs:subClassOf [ a owl:Restriction ;
            owl:maxQualifiedCardinality 1 ;
            owl:onClass linkml:String ;
            owl:onProperty linkml:identifier_pattern ],
        [ a owl:Restriction ;
            owl:maxQualifiedCardinality 1 ;
            owl:onClass linkml:Uriorcurie ;
            owl:onProperty linkml:source_ontology ] ;
    skos:definition "A query that is used on an enum expression to dynamically obtain a set of permissivle values via a query that matches on properties of the external concepts" .

linkml:equals_number a owl:ObjectProperty,
        linkml:SlotDefinition ;
    rdfs:label "equals_number" ;
    rdfs:range linkml:Integer ;
    rdfs:subPropertyOf linkml:list_value_specification_constant ;
    skos:definition "the slot must have range of a number and the value of the slot must equal the specified value" .

linkml:equals_string a owl:ObjectProperty,
        linkml:SlotDefinition ;
    rdfs:label "equals_string" ;
    rdfs:range linkml:String ;
    rdfs:subPropertyOf linkml:list_value_specification_constant ;
    skos:definition "the slot must have range string and the value of the slot must equal the specified value" .

linkml:equals_string_in a owl:ObjectProperty,
        linkml:SlotDefinition ;
    rdfs:label "equals_string_in" ;
    rdfs:range linkml:String ;
    rdfs:subPropertyOf linkml:list_value_specification_constant ;
    skos:definition "the slot must have range string and the value of the slot must equal one of the specified values" .

linkml:implicit_prefix a owl:ObjectProperty,
        linkml:SlotDefinition ;
    rdfs:label "implicit_prefix" ;
    rdfs:domain linkml:SlotExpression ;
    rdfs:range linkml:String ;
    skos:definition "Causes the slot value to be interpreted as a uriorcurie after prefixing with this string" .

linkml:maximum_value a owl:ObjectProperty,
        linkml:SlotDefinition ;
    rdfs:label "maximum_value" ;
    rdfs:domain linkml:SlotDefinition ;
    rdfs:range linkml:Integer ;
    skos:altLabel "high value" ;
    skos:definition "for slots with ranges of type number, the value must be equal to or lowe than this" .

linkml:minimum_value a owl:ObjectProperty,
        linkml:SlotDefinition ;
    rdfs:label "minimum_value" ;
    rdfs:domain linkml:SlotDefinition ;
    rdfs:range linkml:Integer ;
    skos:altLabel "low value" ;
    skos:definition "for slots with ranges of type number, the value must be equal to or higher than this" .

linkml:pattern a owl:ObjectProperty,
        linkml:SlotDefinition ;
    rdfs:label "pattern" ;
    rdfs:domain linkml:Definition ;
    rdfs:range linkml:String ;
    skos:definition "the string value of the slot must conform to this regular expression expressed in the string" .

linkml:relational_logical_characteristic a owl:ObjectProperty,
        linkml:SlotDefinition ;
    rdfs:label "relational_logical_characteristic" ;
    rdfs:domain linkml:SlotDefinition ;
    rdfs:range linkml:Boolean ;
    skos:definition "An abstract grouping for metaslots that describe logical properties of a slot" .

linkml:structured_pattern a owl:ObjectProperty,
        linkml:SlotDefinition ;
    rdfs:label "structured_pattern" ;
    rdfs:domain linkml:Definition ;
    rdfs:range linkml:PatternExpression ;
    rdfs:seeAlso "https://linkml.io/linkml/schemas/constraints.html#structured-patterns" ;
    skos:definition "the string value of the slot must conform to the regular expression in the pattern expression" .

linkml:PathExpression a owl:Class,
        linkml:ClassDefinition ;
    rdfs:label "path_expression" ;
    rdfs:subClassOf [ a owl:Restriction ;
            owl:maxQualifiedCardinality 1 ;
            owl:onClass linkml:String ;
            owl:onProperty linkml:deprecated ],
        [ a owl:Restriction ;
            owl:maxQualifiedCardinality 1 ;
            owl:onClass linkml:Uriorcurie ;
            owl:onProperty oslc:modifiedBy ],
        [ a owl:Restriction ;
            owl:allValuesFrom linkml:Extension ;
            owl:onProperty linkml:extensions ],
        [ a owl:Restriction ;
            owl:allValuesFrom linkml:String ;
            owl:onProperty skos:note ],
        [ a owl:Restriction ;
            owl:maxQualifiedCardinality 1 ;
            owl:onClass linkml:Boolean ;
            owl:onProperty linkml:reversed ],
        [ a owl:Restriction ;
            owl:maxQualifiedCardinality 1 ;
            owl:onClass linkml:Uriorcurie ;
            owl:onProperty dcterms:source ],
        [ a owl:Restriction ;
            owl:allValuesFrom linkml:PathExpression ;
            owl:onProperty linkml:any_of ],
        [ a owl:Restriction ;
            owl:maxQualifiedCardinality 1 ;
            owl:onClass linkml:AnonymousClassExpression ;
            owl:onProperty linkml:range_expression ],
        [ a owl:Restriction ;
            owl:allValuesFrom linkml:Uriorcurie ;
            owl:onProperty skos:relatedMatch ],
        [ a owl:Restriction ;
            owl:allValuesFrom linkml:String ;
            owl:onProperty skos:altLabel ],
        [ a owl:Restriction ;
            owl:allValuesFrom linkml:PathExpression ;
            owl:onProperty linkml:none_of ],
        [ a owl:Restriction ;
            owl:allValuesFrom linkml:Example ;
            owl:onProperty linkml:examples ],
        [ a owl:Restriction ;
            owl:allValuesFrom linkml:Annotation ;
            owl:onProperty linkml:annotations ],
        [ a owl:Restriction ;
            owl:allValuesFrom linkml:String ;
            owl:onProperty linkml:todos ],
        [ a owl:Restriction ;
            owl:allValuesFrom linkml:String ;
            owl:onProperty skos:editorialNote ],
        [ a owl:Restriction ;
            owl:maxQualifiedCardinality 1 ;
            owl:onClass linkml:Uriorcurie ;
            owl:onProperty bibo:status ],
        [ a owl:Restriction ;
            owl:maxQualifiedCardinality 1 ;
            owl:onClass linkml:Datetime ;
            owl:onProperty pav:createdOn ],
        [ a owl:Restriction ;
            owl:allValuesFrom linkml:PathExpression ;
            owl:onProperty linkml:exactly_one_of ],
        [ a owl:Restriction ;
            owl:maxQualifiedCardinality 1 ;
            owl:onClass linkml:String ;
            owl:onProperty skos:definition ],
        [ a owl:Restriction ;
            owl:maxQualifiedCardinality 1 ;
            owl:onClass linkml:String ;
            owl:onProperty linkml:imported_from ],
        [ a owl:Restriction ;
            owl:maxQualifiedCardinality 1 ;
            owl:onClass linkml:Integer ;
            owl:onProperty sh:order ],
        [ a owl:Restriction ;
            owl:maxQualifiedCardinality 1 ;
            owl:onClass linkml:Uriorcurie ;
            owl:onProperty linkml:deprecated_element_has_exact_replacement ],
        [ a owl:Restriction ;
            owl:allValuesFrom linkml:Uriorcurie ;
            owl:onProperty rdfs:seeAlso ],
        [ a owl:Restriction ;
            owl:allValuesFrom linkml:Uriorcurie ;
            owl:onProperty skos:broadMatch ],
        [ a owl:Restriction ;
            owl:maxQualifiedCardinality 1 ;
            owl:onClass linkml:Uriorcurie ;
            owl:onProperty pav:createdBy ],
        [ a owl:Restriction ;
            owl:allValuesFrom linkml:SubsetDefinition ;
            owl:onProperty OIO:inSubset ],
        [ a owl:Restriction ;
            owl:allValuesFrom linkml:Uriorcurie ;
            owl:onProperty skos:narrowMatch ],
        [ a owl:Restriction ;
            owl:maxQualifiedCardinality 1 ;
            owl:onClass linkml:Uriorcurie ;
            owl:onProperty linkml:deprecated_element_has_possible_replacement ],
        [ a owl:Restriction ;
            owl:allValuesFrom linkml:StructuredAlias ;
            owl:onProperty skosxl:altLabel ],
        [ a owl:Restriction ;
            owl:allValuesFrom linkml:Uriorcurie ;
            owl:onProperty skos:exactMatch ],
        [ a owl:Restriction ;
            owl:maxQualifiedCardinality 1 ;
            owl:onClass linkml:PathExpression ;
            owl:onProperty linkml:followed_by ],
        [ a owl:Restriction ;
            owl:allValuesFrom linkml:PathExpression ;
            owl:onProperty linkml:all_of ],
        [ a owl:Restriction ;
            owl:allValuesFrom linkml:Uriorcurie ;
            owl:onProperty skos:closeMatch ],
        [ a owl:Restriction ;
            owl:maxQualifiedCardinality 1 ;
            owl:onClass linkml:SlotDefinition ;
            owl:onProperty linkml:traverse ],
        [ a owl:Restriction ;
            owl:allValuesFrom linkml:Uriorcurie ;
            owl:onProperty skos:mappingRelation ],
        [ a owl:Restriction ;
            owl:maxQualifiedCardinality 1 ;
            owl:onClass linkml:Datetime ;
            owl:onProperty pav:lastUpdatedOn ],
        [ a owl:Restriction ;
            owl:maxQualifiedCardinality 1 ;
            owl:onClass linkml:String ;
            owl:onProperty schema:inLanguage ],
        [ a owl:Restriction ;
            owl:maxQualifiedCardinality 1 ;
            owl:onClass linkml:Uri ;
            owl:onProperty skos:inScheme ],
        [ a owl:Restriction ;
            owl:allValuesFrom linkml:AltDescription ;
            owl:onProperty linkml:alt_descriptions ],
        [ a owl:Restriction ;
            owl:maxQualifiedCardinality 1 ;
            owl:onClass linkml:String ;
            owl:onProperty dcterms:title ],
        linkml:Annotatable,
        linkml:CommonMetadata,
        linkml:Expression,
        linkml:Extensible ;
    skos:definition "An expression that describes an abstract path from an object to another through a sequence of slot lookups" .

linkml:PresenceEnum a owl:Class,
        linkml:EnumDefinition ;
    rdfs:label "presence_enum" ;
    owl:unionOf ( <https://w3id.org/linkml/PresenceEnum#UNCOMMITTED> <https://w3id.org/linkml/PresenceEnum#PRESENT> <https://w3id.org/linkml/PresenceEnum#ABSENT> ) ;
    linkml:permissible_values <https://w3id.org/linkml/PresenceEnum#ABSENT>,
        <https://w3id.org/linkml/PresenceEnum#PRESENT>,
        <https://w3id.org/linkml/PresenceEnum#UNCOMMITTED> .

linkml:RelationalRoleEnum a owl:Class,
        linkml:EnumDefinition ;
    rdfs:label "relational_role_enum" ;
    owl:unionOf ( rdf:subject rdf:object rdf:predicate <https://w3id.org/linkml/RelationalRoleEnum#NODE> <https://w3id.org/linkml/RelationalRoleEnum#OTHER_ROLE> ) ;
    linkml:permissible_values rdf:object,
        rdf:predicate,
        rdf:subject,
        <https://w3id.org/linkml/RelationalRoleEnum#NODE>,
        <https://w3id.org/linkml/RelationalRoleEnum#OTHER_ROLE> .

linkml:Setting a owl:Class,
        linkml:ClassDefinition ;
    rdfs:label "setting" ;
    rdfs:subClassOf [ a owl:Restriction ;
            owl:onClass linkml:String ;
            owl:onProperty linkml:setting_value ;
            owl:qualifiedCardinality 1 ],
        [ a owl:Restriction ;
            owl:onClass linkml:Ncname ;
            owl:onProperty linkml:setting_key ;
            owl:qualifiedCardinality 1 ] ;
    skos:definition "assignment of a key to a value" .

qudt:unit a owl:ObjectProperty,
        linkml:SlotDefinition ;
    rdfs:label "unit" ;
    rdfs:range linkml:UnitOfMeasure ;
    skos:definition "an encoding of a unit" ;
    skos:exactMatch qudt:unit .

linkml:AnonymousEnumExpression a owl:Class,
        linkml:ClassDefinition ;
    rdfs:label "anonymous_enum_expression" ;
    rdfs:subClassOf [ a owl:Restriction ;
            owl:maxQualifiedCardinality 1 ;
            owl:onClass linkml:PvFormulaOptions ;
            owl:onProperty linkml:pv_formula ],
        [ a owl:Restriction ;
            owl:maxQualifiedCardinality 1 ;
            owl:onClass linkml:String ;
            owl:onProperty linkml:code_set_version ],
        [ a owl:Restriction ;
            owl:maxQualifiedCardinality 1 ;
            owl:onClass linkml:ReachabilityQuery ;
            owl:onProperty linkml:reachable_from ],
        [ a owl:Restriction ;
            owl:maxQualifiedCardinality 1 ;
            owl:onClass linkml:Uriorcurie ;
            owl:onProperty linkml:code_set ],
        [ a owl:Restriction ;
            owl:allValuesFrom linkml:AnonymousEnumExpression ;
            owl:onProperty linkml:minus ],
        [ a owl:Restriction ;
            owl:allValuesFrom linkml:Uriorcurie ;
            owl:onProperty linkml:concepts ],
        [ a owl:Restriction ;
            owl:maxQualifiedCardinality 1 ;
            owl:onClass linkml:String ;
            owl:onProperty linkml:code_set_tag ],
        [ a owl:Restriction ;
            owl:maxQualifiedCardinality 1 ;
            owl:onClass linkml:MatchQuery ;
            owl:onProperty linkml:matches ],
        [ a owl:Restriction ;
            owl:allValuesFrom linkml:AnonymousEnumExpression ;
            owl:onProperty linkml:include ],
        [ a owl:Restriction ;
            owl:allValuesFrom linkml:EnumDefinition ;
            owl:onProperty linkml:inherits ],
        [ a owl:Restriction ;
            owl:allValuesFrom linkml:PermissibleValue ;
            owl:onProperty linkml:permissible_values ],
        linkml:EnumExpression ;
    skos:definition "An enum_expression that is not named" .

linkml:PermissibleValue a owl:Class,
        linkml:ClassDefinition ;
    rdfs:label "permissible_value" ;
    rdfs:subClassOf [ a owl:Restriction ;
            owl:allValuesFrom linkml:String ;
            owl:onProperty skos:editorialNote ],
        [ a owl:Restriction ;
            owl:maxQualifiedCardinality 1 ;
            owl:onClass linkml:Integer ;
            owl:onProperty sh:order ],
        [ a owl:Restriction ;
            owl:maxQualifiedCardinality 1 ;
            owl:onClass linkml:Uriorcurie ;
            owl:onProperty oslc:modifiedBy ],
        [ a owl:Restriction ;
            owl:allValuesFrom linkml:StructuredAlias ;
            owl:onProperty skosxl:altLabel ],
        [ a owl:Restriction ;
            owl:onClass linkml:String ;
            owl:onProperty linkml:text ;
            owl:qualifiedCardinality 1 ],
        [ a owl:Restriction ;
            owl:allValuesFrom linkml:SubsetDefinition ;
            owl:onProperty OIO:inSubset ],
        [ a owl:Restriction ;
            owl:maxQualifiedCardinality 1 ;
            owl:onClass linkml:String ;
            owl:onProperty linkml:deprecated ],
        [ a owl:Restriction ;
            owl:allValuesFrom linkml:Uriorcurie ;
            owl:onProperty skos:narrowMatch ],
        [ a owl:Restriction ;
            owl:maxQualifiedCardinality 1 ;
            owl:onClass linkml:String ;
            owl:onProperty schema:inLanguage ],
        [ a owl:Restriction ;
            owl:maxQualifiedCardinality 1 ;
            owl:onClass linkml:Uriorcurie ;
            owl:onProperty linkml:deprecated_element_has_exact_replacement ],
        [ a owl:Restriction ;
            owl:allValuesFrom linkml:PermissibleValue ;
            owl:onProperty linkml:mixins ],
        [ a owl:Restriction ;
            owl:maxQualifiedCardinality 1 ;
            owl:onClass linkml:PermissibleValue ;
            owl:onProperty linkml:is_a ],
        [ a owl:Restriction ;
            owl:allValuesFrom linkml:Example ;
            owl:onProperty linkml:examples ],
        [ a owl:Restriction ;
            owl:maxQualifiedCardinality 1 ;
            owl:onClass linkml:String ;
            owl:onProperty linkml:imported_from ],
        [ a owl:Restriction ;
            owl:allValuesFrom linkml:Uriorcurie ;
            owl:onProperty skos:closeMatch ],
        [ a owl:Restriction ;
            owl:allValuesFrom linkml:Uriorcurie ;
            owl:onProperty skos:exactMatch ],
        [ a owl:Restriction ;
            owl:allValuesFrom linkml:Extension ;
            owl:onProperty linkml:extensions ],
        [ a owl:Restriction ;
            owl:allValuesFrom linkml:Uriorcurie ;
            owl:onProperty skos:mappingRelation ],
        [ a owl:Restriction ;
            owl:maxQualifiedCardinality 1 ;
            owl:onClass linkml:Uriorcurie ;
            owl:onProperty linkml:meaning ],
        [ a owl:Restriction ;
            owl:maxQualifiedCardinality 1 ;
            owl:onClass linkml:Uriorcurie ;
            owl:onProperty linkml:deprecated_element_has_possible_replacement ],
        [ a owl:Restriction ;
            owl:allValuesFrom linkml:String ;
            owl:onProperty linkml:todos ],
        [ a owl:Restriction ;
            owl:allValuesFrom linkml:Uriorcurie ;
            owl:onProperty rdfs:seeAlso ],
        [ a owl:Restriction ;
            owl:allValuesFrom linkml:String ;
            owl:onProperty skos:note ],
        [ a owl:Restriction ;
            owl:maxQualifiedCardinality 1 ;
            owl:onClass linkml:Datetime ;
            owl:onProperty pav:createdOn ],
        [ a owl:Restriction ;
            owl:allValuesFrom linkml:Uriorcurie ;
            owl:onProperty skos:relatedMatch ],
        [ a owl:Restriction ;
            owl:maxQualifiedCardinality 1 ;
            owl:onClass linkml:Uriorcurie ;
            owl:onProperty bibo:status ],
        [ a owl:Restriction ;
            owl:maxQualifiedCardinality 1 ;
            owl:onClass linkml:UnitOfMeasure ;
            owl:onProperty qudt:unit ],
        [ a owl:Restriction ;
            owl:maxQualifiedCardinality 1 ;
            owl:onClass linkml:Datetime ;
            owl:onProperty pav:lastUpdatedOn ],
        [ a owl:Restriction ;
            owl:allValuesFrom linkml:Annotation ;
            owl:onProperty linkml:annotations ],
        [ a owl:Restriction ;
            owl:allValuesFrom linkml:AltDescription ;
            owl:onProperty linkml:alt_descriptions ],
        [ a owl:Restriction ;
            owl:allValuesFrom linkml:Uriorcurie ;
            owl:onProperty skos:broadMatch ],
        [ a owl:Restriction ;
            owl:maxQualifiedCardinality 1 ;
            owl:onClass linkml:Uriorcurie ;
            owl:onProperty pav:createdBy ],
        [ a owl:Restriction ;
            owl:maxQualifiedCardinality 1 ;
            owl:onClass linkml:String ;
            owl:onProperty dcterms:title ],
        [ a owl:Restriction ;
            owl:maxQualifiedCardinality 1 ;
            owl:onClass linkml:Uriorcurie ;
            owl:onProperty dcterms:source ],
        [ a owl:Restriction ;
            owl:allValuesFrom linkml:String ;
            owl:onProperty skos:altLabel ],
        [ a owl:Restriction ;
            owl:maxQualifiedCardinality 1 ;
            owl:onClass linkml:String ;
            owl:onProperty skos:definition ],
        [ a owl:Restriction ;
            owl:maxQualifiedCardinality 1 ;
            owl:onClass linkml:Uri ;
            owl:onProperty skos:inScheme ],
        linkml:Annotatable,
        linkml:CommonMetadata,
        linkml:Extensible ;
    skos:altLabel "PV" ;
    skos:closeMatch skos:Concept ;
    skos:definition "a permissible value, accompanied by intended text and an optional mapping to a concept URI" .

linkml:PvFormulaOptions a owl:Class,
        linkml:EnumDefinition ;
    rdfs:label "pv_formula_options" ;
    owl:unionOf ( <https://w3id.org/linkml/PvFormulaOptions#CODE> <https://w3id.org/linkml/PvFormulaOptions#CURIE> <https://w3id.org/linkml/PvFormulaOptions#URI> <https://w3id.org/linkml/PvFormulaOptions#FHIR_CODING> ) ;
    linkml:permissible_values <https://w3id.org/linkml/PvFormulaOptions#CODE>,
        <https://w3id.org/linkml/PvFormulaOptions#CURIE>,
        <https://w3id.org/linkml/PvFormulaOptions#FHIR_CODING>,
        <https://w3id.org/linkml/PvFormulaOptions#URI> .

linkml:mixin a owl:ObjectProperty,
        linkml:SlotDefinition ;
    rdfs:label "mixin" ;
    rdfs:domain linkml:Definition ;
    rdfs:range linkml:Boolean ;
    rdfs:seeAlso "https://en.wikipedia.org/wiki/Mixin" ;
    skos:altLabel "trait" ;
    skos:definition "Indicates the class or slot is intended to be inherited from without being an is_a parent. mixins should not be inherited from using is_a, except by other mixins." .

linkml:CommonMetadata a owl:Class,
        linkml:ClassDefinition ;
    rdfs:label "common_metadata" ;
    rdfs:subClassOf [ a owl:Restriction ;
            owl:maxQualifiedCardinality 1 ;
            owl:onClass linkml:String ;
            owl:onProperty linkml:deprecated ],
        [ a owl:Restriction ;
            owl:maxQualifiedCardinality 1 ;
            owl:onClass linkml:String ;
            owl:onProperty dcterms:title ],
        [ a owl:Restriction ;
            owl:allValuesFrom linkml:AltDescription ;
            owl:onProperty linkml:alt_descriptions ],
        [ a owl:Restriction ;
            owl:allValuesFrom linkml:String ;
            owl:onProperty linkml:todos ],
        [ a owl:Restriction ;
            owl:allValuesFrom linkml:Uriorcurie ;
            owl:onProperty skos:closeMatch ],
        [ a owl:Restriction ;
            owl:allValuesFrom linkml:Uriorcurie ;
            owl:onProperty skos:broadMatch ],
        [ a owl:Restriction ;
            owl:allValuesFrom linkml:String ;
            owl:onProperty skos:editorialNote ],
        [ a owl:Restriction ;
            owl:maxQualifiedCardinality 1 ;
            owl:onClass linkml:Uriorcurie ;
            owl:onProperty pav:createdBy ],
        [ a owl:Restriction ;
            owl:maxQualifiedCardinality 1 ;
            owl:onClass linkml:Datetime ;
            owl:onProperty pav:lastUpdatedOn ],
        [ a owl:Restriction ;
            owl:allValuesFrom linkml:Uriorcurie ;
            owl:onProperty rdfs:seeAlso ],
        [ a owl:Restriction ;
            owl:allValuesFrom linkml:StructuredAlias ;
            owl:onProperty skosxl:altLabel ],
        [ a owl:Restriction ;
            owl:maxQualifiedCardinality 1 ;
            owl:onClass linkml:Uriorcurie ;
            owl:onProperty oslc:modifiedBy ],
        [ a owl:Restriction ;
            owl:allValuesFrom linkml:Uriorcurie ;
            owl:onProperty skos:exactMatch ],
        [ a owl:Restriction ;
            owl:allValuesFrom linkml:Example ;
            owl:onProperty linkml:examples ],
        [ a owl:Restriction ;
            owl:allValuesFrom linkml:Uriorcurie ;
            owl:onProperty skos:relatedMatch ],
        [ a owl:Restriction ;
            owl:maxQualifiedCardinality 1 ;
            owl:onClass linkml:Datetime ;
            owl:onProperty pav:createdOn ],
        [ a owl:Restriction ;
            owl:maxQualifiedCardinality 1 ;
            owl:onClass linkml:String ;
            owl:onProperty schema:inLanguage ],
        [ a owl:Restriction ;
            owl:allValuesFrom linkml:Uriorcurie ;
            owl:onProperty skos:mappingRelation ],
        [ a owl:Restriction ;
            owl:allValuesFrom linkml:String ;
            owl:onProperty skos:altLabel ],
        [ a owl:Restriction ;
            owl:allValuesFrom linkml:String ;
            owl:onProperty skos:note ],
        [ a owl:Restriction ;
            owl:maxQualifiedCardinality 1 ;
            owl:onClass linkml:Uriorcurie ;
            owl:onProperty bibo:status ],
        [ a owl:Restriction ;
            owl:maxQualifiedCardinality 1 ;
            owl:onClass linkml:Integer ;
            owl:onProperty sh:order ],
        [ a owl:Restriction ;
            owl:maxQualifiedCardinality 1 ;
            owl:onClass linkml:String ;
            owl:onProperty skos:definition ],
        [ a owl:Restriction ;
            owl:maxQualifiedCardinality 1 ;
            owl:onClass linkml:Uriorcurie ;
            owl:onProperty linkml:deprecated_element_has_exact_replacement ],
        [ a owl:Restriction ;
            owl:allValuesFrom linkml:SubsetDefinition ;
            owl:onProperty OIO:inSubset ],
        [ a owl:Restriction ;
            owl:maxQualifiedCardinality 1 ;
            owl:onClass linkml:Uriorcurie ;
            owl:onProperty dcterms:source ],
        [ a owl:Restriction ;
            owl:maxQualifiedCardinality 1 ;
            owl:onClass linkml:Uri ;
            owl:onProperty skos:inScheme ],
        [ a owl:Restriction ;
            owl:allValuesFrom linkml:Uriorcurie ;
            owl:onProperty skos:narrowMatch ],
        [ a owl:Restriction ;
            owl:maxQualifiedCardinality 1 ;
            owl:onClass linkml:String ;
            owl:onProperty linkml:imported_from ],
        [ a owl:Restriction ;
            owl:maxQualifiedCardinality 1 ;
            owl:onClass linkml:Uriorcurie ;
            owl:onProperty linkml:deprecated_element_has_possible_replacement ],
        linkml:mixin ;
    skos:definition "Generic metadata shared across definitions" .

linkml:PatternExpression a owl:Class,
        linkml:ClassDefinition ;
    rdfs:label "pattern_expression" ;
    rdfs:subClassOf [ a owl:Restriction ;
            owl:allValuesFrom linkml:Annotation ;
            owl:onProperty linkml:annotations ],
        [ a owl:Restriction ;
            owl:allValuesFrom linkml:String ;
            owl:onProperty skos:editorialNote ],
        [ a owl:Restriction ;
            owl:maxQualifiedCardinality 1 ;
            owl:onClass linkml:String ;
            owl:onProperty linkml:syntax ],
        [ a owl:Restriction ;
            owl:maxQualifiedCardinality 1 ;
            owl:onClass linkml:Uriorcurie ;
            owl:onProperty dcterms:source ],
        [ a owl:Restriction ;
            owl:allValuesFrom linkml:Uriorcurie ;
            owl:onProperty skos:mappingRelation ],
        [ a owl:Restriction ;
            owl:allValuesFrom linkml:Uriorcurie ;
            owl:onProperty rdfs:seeAlso ],
        [ a owl:Restriction ;
            owl:allValuesFrom linkml:Example ;
            owl:onProperty linkml:examples ],
        [ a owl:Restriction ;
            owl:maxQualifiedCardinality 1 ;
            owl:onClass linkml:Uri ;
            owl:onProperty skos:inScheme ],
        [ a owl:Restriction ;
            owl:allValuesFrom linkml:String ;
            owl:onProperty skos:altLabel ],
        [ a owl:Restriction ;
            owl:allValuesFrom linkml:Uriorcurie ;
            owl:onProperty skos:exactMatch ],
        [ a owl:Restriction ;
            owl:maxQualifiedCardinality 1 ;
            owl:onClass linkml:String ;
            owl:onProperty linkml:deprecated ],
        [ a owl:Restriction ;
            owl:maxQualifiedCardinality 1 ;
            owl:onClass linkml:Uriorcurie ;
            owl:onProperty oslc:modifiedBy ],
        [ a owl:Restriction ;
            owl:allValuesFrom linkml:String ;
            owl:onProperty skos:note ],
        [ a owl:Restriction ;
            owl:maxQualifiedCardinality 1 ;
            owl:onClass linkml:Datetime ;
            owl:onProperty pav:lastUpdatedOn ],
        [ a owl:Restriction ;
            owl:maxQualifiedCardinality 1 ;
            owl:onClass linkml:Uriorcurie ;
            owl:onProperty pav:createdBy ],
        [ a owl:Restriction ;
            owl:allValuesFrom linkml:Uriorcurie ;
            owl:onProperty skos:relatedMatch ],
        [ a owl:Restriction ;
            owl:allValuesFrom linkml:AltDescription ;
            owl:onProperty linkml:alt_descriptions ],
        [ a owl:Restriction ;
            owl:maxQualifiedCardinality 1 ;
            owl:onClass linkml:String ;
            owl:onProperty schema:inLanguage ],
        [ a owl:Restriction ;
            owl:allValuesFrom linkml:Extension ;
            owl:onProperty linkml:extensions ],
        [ a owl:Restriction ;
            owl:allValuesFrom linkml:Uriorcurie ;
            owl:onProperty skos:narrowMatch ],
        [ a owl:Restriction ;
            owl:maxQualifiedCardinality 1 ;
            owl:onClass linkml:String ;
            owl:onProperty linkml:imported_from ],
        [ a owl:Restriction ;
            owl:maxQualifiedCardinality 1 ;
            owl:onClass linkml:String ;
            owl:onProperty skos:definition ],
        [ a owl:Restriction ;
            owl:allValuesFrom linkml:SubsetDefinition ;
            owl:onProperty OIO:inSubset ],
        [ a owl:Restriction ;
            owl:allValuesFrom linkml:StructuredAlias ;
            owl:onProperty skosxl:altLabel ],
        [ a owl:Restriction ;
            owl:maxQualifiedCardinality 1 ;
            owl:onClass linkml:Boolean ;
            owl:onProperty linkml:interpolated ],
        [ a owl:Restriction ;
            owl:allValuesFrom linkml:String ;
            owl:onProperty linkml:todos ],
        [ a owl:Restriction ;
            owl:allValuesFrom linkml:Uriorcurie ;
            owl:onProperty skos:closeMatch ],
        [ a owl:Restriction ;
            owl:maxQualifiedCardinality 1 ;
            owl:onClass linkml:Datetime ;
            owl:onProperty pav:createdOn ],
        [ a owl:Restriction ;
            owl:maxQualifiedCardinality 1 ;
            owl:onClass linkml:Boolean ;
            owl:onProperty linkml:partial_match ],
        [ a owl:Restriction ;
            owl:allValuesFrom linkml:Uriorcurie ;
            owl:onProperty skos:broadMatch ],
        [ a owl:Restriction ;
            owl:maxQualifiedCardinality 1 ;
            owl:onClass linkml:Uriorcurie ;
            owl:onProperty linkml:deprecated_element_has_possible_replacement ],
        [ a owl:Restriction ;
            owl:maxQualifiedCardinality 1 ;
            owl:onClass linkml:Uriorcurie ;
            owl:onProperty bibo:status ],
        [ a owl:Restriction ;
            owl:maxQualifiedCardinality 1 ;
            owl:onClass linkml:Integer ;
            owl:onProperty sh:order ],
        [ a owl:Restriction ;
            owl:maxQualifiedCardinality 1 ;
            owl:onClass linkml:Uriorcurie ;
            owl:onProperty linkml:deprecated_element_has_exact_replacement ],
        [ a owl:Restriction ;
            owl:maxQualifiedCardinality 1 ;
            owl:onClass linkml:String ;
            owl:onProperty dcterms:title ],
        linkml:Annotatable,
        linkml:CommonMetadata,
        linkml:Extensible ;
    skos:definition "a regular expression pattern used to evaluate conformance of a string" .

linkml:ReachabilityQuery a owl:Class,
        linkml:ClassDefinition ;
    rdfs:label "reachability_query" ;
    rdfs:subClassOf [ a owl:Restriction ;
            owl:maxQualifiedCardinality 1 ;
            owl:onClass linkml:Uriorcurie ;
            owl:onProperty linkml:source_ontology ],
        [ a owl:Restriction ;
            owl:maxQualifiedCardinality 1 ;
            owl:onClass linkml:Boolean ;
            owl:onProperty linkml:is_direct ],
        [ a owl:Restriction ;
            owl:allValuesFrom linkml:Uriorcurie ;
            owl:onProperty linkml:relationship_types ],
        [ a owl:Restriction ;
            owl:maxQualifiedCardinality 1 ;
            owl:onClass linkml:Boolean ;
            owl:onProperty linkml:include_self ],
        [ a owl:Restriction ;
            owl:maxQualifiedCardinality 1 ;
            owl:onClass linkml:Boolean ;
            owl:onProperty linkml:traverse_up ],
        [ a owl:Restriction ;
            owl:allValuesFrom linkml:Uriorcurie ;
            owl:onProperty linkml:source_nodes ] ;
    skos:definition "A query that is used on an enum expression to dynamically obtain a set of permissible values via walking from a set of source nodes to a set of descendants or ancestors over a set of relationship types" .

linkml:UnitOfMeasure a owl:Class,
        linkml:ClassDefinition ;
    rdfs:label "UnitOfMeasure" ;
    rdfs:subClassOf [ a owl:Restriction ;
            owl:maxQualifiedCardinality 1 ;
            owl:onClass linkml:String ;
            owl:onProperty qudt:iec61360Code ],
        [ a owl:Restriction ;
            owl:maxQualifiedCardinality 1 ;
            owl:onClass linkml:String ;
            owl:onProperty qudt:ucumCode ],
        [ a owl:Restriction ;
            owl:maxQualifiedCardinality 1 ;
            owl:onClass linkml:Uriorcurie ;
            owl:onProperty qudt:hasQuantityKind ],
        [ a owl:Restriction ;
            owl:allValuesFrom linkml:Uriorcurie ;
            owl:onProperty skos:exactMatch ],
        [ a owl:Restriction ;
            owl:maxQualifiedCardinality 1 ;
            owl:onClass linkml:String ;
            owl:onProperty rdfs:label ],
        [ a owl:Restriction ;
            owl:maxQualifiedCardinality 1 ;
            owl:onClass linkml:String ;
            owl:onProperty qudt:symbol ],
        [ a owl:Restriction ;
            owl:maxQualifiedCardinality 1 ;
            owl:onClass linkml:String ;
            owl:onProperty linkml:derivation ],
        [ a owl:Restriction ;
            owl:maxQualifiedCardinality 1 ;
            owl:onClass linkml:String ;
            owl:onProperty qudt:abbreviation ] ;
    skos:definition "A unit of measure, or unit, is a particular quantity value that has been chosen as a scale for measuring other quantities the same kind (more generally of equivalent dimension)." ;
    skos:exactMatch qudt:Unit .

linkml:all_of a owl:ObjectProperty,
        linkml:SlotDefinition ;
    rdfs:label "all_of" ;
    rdfs:range linkml:Expression ;
    rdfs:seeAlso "https://w3id.org/linkml/docs/specification/05validation/#rules" ;
    rdfs:subPropertyOf linkml:boolean_slot ;
    skos:definition "holds if all of the expressions hold" ;
    skos:exactMatch sh:and .

linkml:alt_descriptions a owl:ObjectProperty,
        linkml:SlotDefinition ;
    rdfs:label "alt_descriptions" ;
    rdfs:domain linkml:Element ;
    rdfs:range linkml:AltDescription ;
    skos:altLabel "alternate definitions" ;
    skos:definition "A sourced alternative description for an element" .

linkml:any_of a owl:ObjectProperty,
        linkml:SlotDefinition ;
    rdfs:label "any_of" ;
    rdfs:range linkml:Expression ;
    rdfs:seeAlso "https://w3id.org/linkml/docs/specification/05validation/#rules" ;
    rdfs:subPropertyOf linkml:boolean_slot ;
    skos:definition "holds if at least one of the expressions hold" ;
    skos:exactMatch sh:or .

linkml:deprecated a owl:ObjectProperty,
        linkml:SlotDefinition ;
    rdfs:label "deprecated" ;
    rdfs:domain linkml:Element ;
    rdfs:range linkml:String ;
    skos:closeMatch owl:deprecated ;
    skos:definition "Description of why and when this element will no longer be used" ;
    skos:note "note that linkml does not use a boolean to indicate deprecation status - the presence of a string value in this field is sufficient to indicate deprecation." .

linkml:deprecated_element_has_exact_replacement a owl:ObjectProperty,
        linkml:SlotDefinition ;
    rdfs:label "deprecated element has exact replacement" ;
    rdfs:range linkml:Uriorcurie ;
    skos:definition "When an element is deprecated, it can be automatically replaced by this uri or curie" ;
    skos:exactMatch IAO:0100001 .

linkml:deprecated_element_has_possible_replacement a owl:ObjectProperty,
        linkml:SlotDefinition ;
    rdfs:label "deprecated element has possible replacement" ;
    rdfs:range linkml:Uriorcurie ;
    skos:definition "When an element is deprecated, it can be potentially replaced by this uri or curie" ;
    skos:exactMatch OIO:consider .

linkml:exactly_one_of a owl:ObjectProperty,
        linkml:SlotDefinition ;
    rdfs:label "exactly_one_of" ;
    rdfs:range linkml:Expression ;
    rdfs:seeAlso "https://w3id.org/linkml/docs/specification/05validation/#rules" ;
    rdfs:subPropertyOf linkml:boolean_slot ;
    skos:definition "holds if only one of the expressions hold" ;
    skos:exactMatch sh:xone .

linkml:examples a owl:ObjectProperty,
        linkml:SlotDefinition ;
    rdfs:label "examples" ;
    rdfs:domain linkml:Element ;
    rdfs:range linkml:Example ;
    skos:closeMatch vann:example ;
    skos:definition "example usages of an element" .

linkml:imported_from a owl:ObjectProperty,
        linkml:SlotDefinition ;
    rdfs:label "imported_from" ;
    rdfs:domain linkml:Element ;
    rdfs:range linkml:String ;
    skos:definition "the imports entry that this element was derived from.  Empty means primary source" .

linkml:list_value_specification_constant a owl:ObjectProperty,
        linkml:SlotDefinition ;
    rdfs:label "list_value_specification_constant" ;
    rdfs:range linkml:String ;
    skos:definition "Grouping for metamodel slots that constrain members of a multivalued slot value to equal a specified constant" .

linkml:none_of a owl:ObjectProperty,
        linkml:SlotDefinition ;
    rdfs:label "none_of" ;
    rdfs:range linkml:Expression ;
    rdfs:seeAlso "https://w3id.org/linkml/docs/specification/05validation/#rules" ;
    rdfs:subPropertyOf linkml:boolean_slot ;
    skos:definition "holds if none of the expressions hold" ;
    skos:exactMatch sh:not .

linkml:todos a owl:ObjectProperty,
        linkml:SlotDefinition ;
    rdfs:label "todos" ;
    rdfs:domain linkml:Element ;
    rdfs:range linkml:String ;
    skos:definition "Outstanding issues that needs resolution" .

oslc:modifiedBy a owl:ObjectProperty,
        linkml:SlotDefinition ;
    rdfs:label "modified_by" ;
    rdfs:domain linkml:Element ;
    rdfs:range linkml:Uriorcurie ;
    skos:definition "agent that modified the element" ;
    skos:exactMatch oslc:modifiedBy .

dcterms:source a owl:ObjectProperty,
        linkml:SlotDefinition ;
    rdfs:label "source" ;
    rdfs:domain linkml:Element ;
    rdfs:range linkml:Uriorcurie ;
    skos:altLabel "derived from",
        "origin" ;
    skos:closeMatch schema:isBasedOn,
        prov:wasDerivedFrom ;
    skos:definition "A related resource from which the element is derived." ;
    skos:exactMatch dcterms:source ;
    skos:note "The described resource may be derived from the related resource in whole or in part" .

dcterms:title a owl:ObjectProperty,
        linkml:SlotDefinition ;
    rdfs:label "title" ;
    rdfs:domain linkml:Element ;
    rdfs:range linkml:String ;
    skos:altLabel "long name" ;
    skos:definition "A concise human-readable display label for the element. The title should mirror the name, and should use ordinary textual punctuation." ;
    skos:exactMatch dcterms:title .

bibo:status a owl:ObjectProperty,
        linkml:SlotDefinition ;
    rdfs:label "status" ;
    rdfs:domain linkml:Element ;
    rdfs:range linkml:Uriorcurie ;
    rdfs:seeAlso "https://www.hl7.org/fhir/valueset-publication-status.html",
        "https://www.hl7.org/fhir/versions.html#std-process" ;
    skos:altLabel "workflow status" ;
    skos:definition "status of the element" ;
    skos:exactMatch bibo:status ;
    linkml:examples "Example(value='bibo:draft', description=None)" .

pav:createdBy a owl:ObjectProperty,
        linkml:SlotDefinition ;
    rdfs:label "created_by" ;
    rdfs:domain linkml:Element ;
    rdfs:range linkml:Uriorcurie ;
    skos:definition "agent that created the element" ;
    skos:exactMatch pav:createdBy .

pav:createdOn a owl:ObjectProperty,
        linkml:SlotDefinition ;
    rdfs:label "created_on" ;
    rdfs:domain linkml:Element ;
    rdfs:range linkml:Datetime ;
    skos:definition "time at which the element was created" ;
    skos:exactMatch pav:createdOn .

pav:lastUpdatedOn a owl:ObjectProperty,
        linkml:SlotDefinition ;
    rdfs:label "last_updated_on" ;
    rdfs:domain linkml:Element ;
    rdfs:range linkml:Datetime ;
    skos:definition "time at which the element was last updated" ;
    skos:exactMatch pav:lastUpdatedOn .

schema:inLanguage a owl:ObjectProperty,
        linkml:SlotDefinition ;
    rdfs:label "in_language" ;
    dcterms:conformsTo "https://www.rfc-editor.org/rfc/bcp/bcp47.txt" ;
    rdfs:range linkml:String ;
    skos:definition "the primary language used in the sources" ;
    skos:exactMatch schema:inLanguage ;
    skos:note "Recommended to use a string from IETF BCP 47" .

OIO:inSubset a owl:ObjectProperty,
        linkml:SlotDefinition ;
    rdfs:label "in_subset" ;
    rdfs:domain linkml:Element ;
    rdfs:range linkml:SubsetDefinition ;
    skos:definition "used to indicate membership of a term in a defined subset of terms used for a particular domain or application." ;
    skos:exactMatch OIO:inSubset ;
    skos:note "an example of use in the translator_minimal subset in the biolink model, holding the minimal set of predicates used in a translator knowledge graph" .

rdfs:seeAlso a owl:ObjectProperty,
        linkml:SlotDefinition ;
    rdfs:label "see_also" ;
    rdfs:domain linkml:Element ;
    rdfs:range linkml:Uriorcurie ;
    skos:definition "A list of related entities or URLs that may be of relevance" ;
    skos:exactMatch rdfs:seeAlso .

skos:broadMatch a owl:ObjectProperty,
        linkml:SlotDefinition ;
    rdfs:label "broad mappings" ;
    rdfs:range linkml:Uriorcurie ;
    rdfs:subPropertyOf skos:mappingRelation ;
    skos:definition "A list of terms from different schemas or terminology systems that have broader meaning." ;
    skos:exactMatch skos:broadMatch .

skos:closeMatch a owl:ObjectProperty,
        linkml:SlotDefinition ;
    rdfs:label "close mappings" ;
    rdfs:range linkml:Uriorcurie ;
    rdfs:subPropertyOf skos:mappingRelation ;
    skos:definition "A list of terms from different schemas or terminology systems that have close meaning." ;
    skos:exactMatch skos:closeMatch .

skos:definition a owl:ObjectProperty,
        linkml:SlotDefinition ;
    rdfs:label "description" ;
    rdfs:domain linkml:Element ;
    rdfs:range linkml:String ;
    skos:altLabel "definition" ;
    skos:definition "a textual description of the element's purpose and use" ;
    skos:exactMatch dcterms:description,
        schema:description,
        skos:definition .

skos:editorialNote a owl:ObjectProperty,
        linkml:SlotDefinition ;
    rdfs:label "notes" ;
    rdfs:domain linkml:Element ;
    rdfs:range linkml:String ;
    skos:definition "editorial notes about an element intended primarily for internal consumption" ;
    skos:exactMatch skos:editorialNote .

skos:inScheme a owl:ObjectProperty,
        linkml:SlotDefinition ;
    rdfs:label "from_schema" ;
    rdfs:domain linkml:Element ;
    rdfs:range linkml:Uri ;
    skos:definition "id of the schema that defined the element" ;
    skos:editorialNote "A stronger model would be range schema_definition, but this doesn't address the import model" ;
    skos:exactMatch skos:inScheme .

skos:narrowMatch a owl:ObjectProperty,
        linkml:SlotDefinition ;
    rdfs:label "narrow mappings" ;
    rdfs:range linkml:Uriorcurie ;
    rdfs:subPropertyOf skos:mappingRelation ;
    skos:definition "A list of terms from different schemas or terminology systems that have narrower meaning." ;
    skos:exactMatch skos:narrowMatch .

skos:note a owl:ObjectProperty,
        linkml:SlotDefinition ;
    rdfs:label "comments" ;
    rdfs:domain linkml:Element ;
    rdfs:range linkml:String ;
    skos:definition "notes and comments about an element intended primarily for external consumption" ;
    skos:exactMatch rdfs:comment,
        skos:note .

skosxl:altLabel a owl:ObjectProperty,
        linkml:SlotDefinition ;
    rdfs:label "structured_aliases" ;
    rdfs:range linkml:StructuredAlias ;
    rdfs:seeAlso "linkml:aliases" ;
    skos:definition "A list of structured_alias objects, used to provide aliases in conjunction with additional metadata." ;
    skos:exactMatch skosxl:altLabel .

sh:order a owl:ObjectProperty,
        linkml:SlotDefinition ;
    rdfs:label "rank" ;
    rdfs:range linkml:Integer ;
    skos:altLabel "display order",
        "order",
        "precedence" ;
    skos:definition "the relative order in which the element occurs, lower values are given precedence" ;
    skos:exactMatch qb:order,
        qudt:order,
        sh:order ;
    skos:note "the rank of an element does not affect the semantics" .

linkml:EnumDefinition a owl:Class,
        linkml:ClassDefinition ;
    rdfs:label "enum_definition" ;
    rdfs:subClassOf [ a owl:Restriction ;
            owl:maxQualifiedCardinality 1 ;
            owl:onClass linkml:Uriorcurie ;
            owl:onProperty linkml:enum_uri ],
        [ a owl:Restriction ;
            owl:allValuesFrom linkml:PermissibleValue ;
            owl:onProperty linkml:permissible_values ],
        [ a owl:Restriction ;
            owl:allValuesFrom linkml:Uriorcurie ;
            owl:onProperty linkml:concepts ],
        [ a owl:Restriction ;
            owl:allValuesFrom linkml:AnonymousEnumExpression ;
            owl:onProperty linkml:include ],
        [ a owl:Restriction ;
            owl:maxQualifiedCardinality 1 ;
            owl:onClass linkml:PvFormulaOptions ;
            owl:onProperty linkml:pv_formula ],
        [ a owl:Restriction ;
            owl:allValuesFrom linkml:AnonymousEnumExpression ;
            owl:onProperty linkml:minus ],
        [ a owl:Restriction ;
            owl:allValuesFrom linkml:EnumDefinition ;
            owl:onProperty linkml:inherits ],
        [ a owl:Restriction ;
            owl:maxQualifiedCardinality 1 ;
            owl:onClass linkml:String ;
            owl:onProperty linkml:code_set_version ],
        [ a owl:Restriction ;
            owl:maxQualifiedCardinality 1 ;
            owl:onClass linkml:MatchQuery ;
            owl:onProperty linkml:matches ],
        [ a owl:Restriction ;
            owl:maxQualifiedCardinality 1 ;
            owl:onClass linkml:String ;
            owl:onProperty linkml:code_set_tag ],
        [ a owl:Restriction ;
            owl:maxQualifiedCardinality 1 ;
            owl:onClass linkml:ReachabilityQuery ;
            owl:onProperty linkml:reachable_from ],
        [ a owl:Restriction ;
            owl:maxQualifiedCardinality 1 ;
            owl:onClass linkml:Uriorcurie ;
            owl:onProperty linkml:code_set ],
        linkml:Definition,
        linkml:EnumExpression ;
    skos:altLabel "Terminology Value Set",
        "answer list",
        "concept set",
        "enum",
        "term set",
        "value set" ;
    skos:closeMatch skos:ConceptScheme ;
    skos:definition "an element whose instances must be drawn from a specified set of permissible values" ;
    skos:exactMatch NCIT:C113497,
        qb:HierarchicalCodeList .

linkml:Extensible a owl:Class,
        linkml:ClassDefinition ;
    rdfs:label "extensible" ;
    rdfs:subClassOf [ a owl:Restriction ;
            owl:allValuesFrom linkml:Extension ;
            owl:onProperty linkml:extensions ],
        linkml:mixin ;
    skos:definition "mixin for classes that support extension" .

linkml:TypeDefinition a owl:Class,
        linkml:ClassDefinition ;
    rdfs:label "type_definition" ;
    rdfs:subClassOf [ a owl:Restriction ;
            owl:maxQualifiedCardinality 1 ;
            owl:onClass linkml:Uriorcurie ;
            owl:onProperty linkml:uri ],
        [ a owl:Restriction ;
            owl:maxQualifiedCardinality 1 ;
            owl:onClass linkml:String ;
            owl:onProperty linkml:pattern ],
        [ a owl:Restriction ;
            owl:maxQualifiedCardinality 1 ;
            owl:onClass linkml:String ;
            owl:onProperty linkml:repr ],
        [ a owl:Restriction ;
            owl:maxQualifiedCardinality 1 ;
            owl:onClass linkml:TypeDefinition ;
            owl:onProperty linkml:typeof ],
        [ a owl:Restriction ;
            owl:allValuesFrom linkml:AnonymousTypeExpression ;
            owl:onProperty linkml:all_of ],
        [ a owl:Restriction ;
            owl:allValuesFrom linkml:AnonymousTypeExpression ;
            owl:onProperty linkml:none_of ],
        [ a owl:Restriction ;
            owl:allValuesFrom linkml:AnonymousTypeExpression ;
            owl:onProperty linkml:any_of ],
        [ a owl:Restriction ;
            owl:allValuesFrom linkml:String ;
            owl:onProperty linkml:equals_string_in ],
        [ a owl:Restriction ;
            owl:allValuesFrom linkml:TypeDefinition ;
            owl:onProperty linkml:union_of ],
        [ a owl:Restriction ;
            owl:allValuesFrom linkml:AnonymousTypeExpression ;
            owl:onProperty linkml:exactly_one_of ],
        [ a owl:Restriction ;
            owl:maxQualifiedCardinality 1 ;
            owl:onClass linkml:String ;
            owl:onProperty linkml:implicit_prefix ],
        [ a owl:Restriction ;
            owl:maxQualifiedCardinality 1 ;
            owl:onClass linkml:Integer ;
            owl:onProperty linkml:minimum_value ],
        [ a owl:Restriction ;
            owl:maxQualifiedCardinality 1 ;
            owl:onClass linkml:Integer ;
            owl:onProperty linkml:maximum_value ],
        [ a owl:Restriction ;
            owl:maxQualifiedCardinality 1 ;
            owl:onClass linkml:UnitOfMeasure ;
            owl:onProperty qudt:unit ],
        [ a owl:Restriction ;
            owl:maxQualifiedCardinality 1 ;
            owl:onClass linkml:String ;
            owl:onProperty linkml:base ],
        [ a owl:Restriction ;
            owl:maxQualifiedCardinality 1 ;
            owl:onClass linkml:String ;
            owl:onProperty linkml:equals_string ],
        [ a owl:Restriction ;
            owl:maxQualifiedCardinality 1 ;
            owl:onClass linkml:Integer ;
            owl:onProperty linkml:equals_number ],
        [ a owl:Restriction ;
            owl:maxQualifiedCardinality 1 ;
            owl:onClass linkml:PatternExpression ;
            owl:onProperty linkml:structured_pattern ],
        linkml:Element,
        linkml:TypeExpression ;
    skos:definition "an element that whose instances are atomic scalar values that can be mapped to primitive types" .

linkml:annotations a owl:ObjectProperty,
        linkml:SlotDefinition ;
    rdfs:label "annotations" ;
    rdfs:domain linkml:Annotatable ;
    rdfs:range linkml:Annotation ;
    rdfs:subPropertyOf linkml:extensions ;
    skos:definition "a collection of tag/text tuples with the semantics of OWL Annotation" .

skos:altLabel a owl:ObjectProperty,
        linkml:SlotDefinition .

linkml:AltDescription a owl:Class,
        linkml:ClassDefinition ;
    rdfs:label "alt_description" ;
    rdfs:subClassOf [ a owl:Restriction ;
            owl:onClass linkml:String ;
            owl:onProperty linkml:source ;
            owl:qualifiedCardinality 1 ],
        [ a owl:Restriction ;
            owl:onClass linkml:String ;
            owl:onProperty linkml:description ;
            owl:qualifiedCardinality 1 ] ;
    skos:altLabel "structured description" ;
    skos:definition "an attributed description" .

linkml:Annotatable a owl:Class,
        linkml:ClassDefinition ;
    rdfs:label "annotatable" ;
    rdfs:subClassOf [ a owl:Restriction ;
            owl:allValuesFrom linkml:Annotation ;
            owl:onProperty linkml:annotations ],
        linkml:mixin ;
    skos:definition "mixin for classes that support annotations" .

linkml:Annotation a owl:Class,
        linkml:ClassDefinition ;
    rdfs:label "annotation" ;
    rdfs:subClassOf [ a owl:Restriction ;
            owl:allValuesFrom linkml:Annotation ;
            owl:onProperty linkml:annotations ],
        linkml:Annotatable,
        linkml:Extension ;
    skos:definition "a tag/value pair with the semantics of OWL Annotation" .

linkml:AnonymousTypeExpression a owl:Class,
        linkml:ClassDefinition ;
    rdfs:label "anonymous_type_expression" ;
    rdfs:subClassOf [ a owl:Restriction ;
            owl:maxQualifiedCardinality 1 ;
            owl:onClass linkml:PatternExpression ;
            owl:onProperty linkml:structured_pattern ],
        [ a owl:Restriction ;
            owl:allValuesFrom linkml:AnonymousTypeExpression ;
            owl:onProperty linkml:all_of ],
        [ a owl:Restriction ;
            owl:allValuesFrom linkml:AnonymousTypeExpression ;
            owl:onProperty linkml:none_of ],
        [ a owl:Restriction ;
            owl:allValuesFrom linkml:AnonymousTypeExpression ;
            owl:onProperty linkml:exactly_one_of ],
        [ a owl:Restriction ;
            owl:maxQualifiedCardinality 1 ;
            owl:onClass linkml:String ;
            owl:onProperty linkml:equals_string ],
        [ a owl:Restriction ;
            owl:maxQualifiedCardinality 1 ;
            owl:onClass linkml:String ;
            owl:onProperty linkml:pattern ],
        [ a owl:Restriction ;
            owl:maxQualifiedCardinality 1 ;
            owl:onClass linkml:Integer ;
            owl:onProperty linkml:minimum_value ],
        [ a owl:Restriction ;
            owl:maxQualifiedCardinality 1 ;
            owl:onClass linkml:Integer ;
            owl:onProperty linkml:maximum_value ],
        [ a owl:Restriction ;
            owl:maxQualifiedCardinality 1 ;
            owl:onClass linkml:String ;
            owl:onProperty linkml:implicit_prefix ],
        [ a owl:Restriction ;
            owl:maxQualifiedCardinality 1 ;
            owl:onClass linkml:UnitOfMeasure ;
            owl:onProperty qudt:unit ],
        [ a owl:Restriction ;
            owl:maxQualifiedCardinality 1 ;
            owl:onClass linkml:Integer ;
            owl:onProperty linkml:equals_number ],
        [ a owl:Restriction ;
            owl:allValuesFrom linkml:String ;
            owl:onProperty linkml:equals_string_in ],
        [ a owl:Restriction ;
            owl:allValuesFrom linkml:AnonymousTypeExpression ;
            owl:onProperty linkml:any_of ],
        linkml:TypeExpression ;
    skos:definition "A type expression that is not a top-level named type definition. Used for nesting." .

linkml:extensions a owl:ObjectProperty,
        linkml:SlotDefinition ;
    rdfs:label "extensions" ;
    rdfs:domain linkml:Extensible ;
    rdfs:range linkml:Extension ;
    skos:definition "a tag/text tuple attached to an arbitrary element" .

skos:relatedMatch a owl:Class,
        owl:ObjectProperty,
        linkml:AliasPredicateEnum,
        linkml:SlotDefinition ;
    rdfs:label "RELATED_SYNONYM",
        "related mappings" ;
    rdfs:range linkml:Uriorcurie ;
    rdfs:subPropertyOf skos:mappingRelation ;
    skos:definition "A list of terms from different schemas or terminology systems that have related meaning." ;
    skos:exactMatch skos:relatedMatch .

linkml:Expression a owl:Class,
        linkml:ClassDefinition ;
    rdfs:label "expression" ;
    rdfs:subClassOf linkml:mixin ;
    skos:definition "general mixin for any class that can represent some form of expression" .

linkml:StructuredAlias a owl:Class,
        linkml:ClassDefinition ;
    rdfs:label "structured_alias" ;
    rdfs:subClassOf [ a owl:Restriction ;
            owl:maxQualifiedCardinality 1 ;
            owl:onClass linkml:String ;
            owl:onProperty linkml:deprecated ],
        [ a owl:Restriction ;
            owl:maxQualifiedCardinality 1 ;
            owl:onClass linkml:String ;
            owl:onProperty linkml:imported_from ],
        [ a owl:Restriction ;
            owl:allValuesFrom linkml:String ;
            owl:onProperty skos:note ],
        [ a owl:Restriction ;
            owl:maxQualifiedCardinality 1 ;
            owl:onClass linkml:Uri ;
            owl:onProperty skos:inScheme ],
        [ a owl:Restriction ;
            owl:maxQualifiedCardinality 1 ;
            owl:onClass linkml:Uriorcurie ;
            owl:onProperty pav:createdBy ],
        [ a owl:Restriction ;
            owl:allValuesFrom linkml:Uriorcurie ;
            owl:onProperty rdfs:seeAlso ],
        [ a owl:Restriction ;
            owl:allValuesFrom linkml:Uriorcurie ;
            owl:onProperty dcterms:subject ],
        [ a owl:Restriction ;
            owl:onClass linkml:String ;
            owl:onProperty skosxl:literalForm ;
            owl:qualifiedCardinality 1 ],
        [ a owl:Restriction ;
            owl:allValuesFrom linkml:Uriorcurie ;
            owl:onProperty skos:broadMatch ],
        [ a owl:Restriction ;
            owl:maxQualifiedCardinality 1 ;
            owl:onClass linkml:Uriorcurie ;
            owl:onProperty linkml:deprecated_element_has_exact_replacement ],
        [ a owl:Restriction ;
            owl:maxQualifiedCardinality 1 ;
            owl:onClass linkml:Datetime ;
            owl:onProperty pav:createdOn ],
        [ a owl:Restriction ;
            owl:allValuesFrom linkml:String ;
            owl:onProperty skos:altLabel ],
        [ a owl:Restriction ;
            owl:allValuesFrom linkml:Uriorcurie ;
            owl:onProperty skos:relatedMatch ],
        [ a owl:Restriction ;
            owl:maxQualifiedCardinality 1 ;
            owl:onClass linkml:String ;
            owl:onProperty schema:inLanguage ],
        [ a owl:Restriction ;
            owl:allValuesFrom linkml:Uriorcurie ;
            owl:onProperty skos:closeMatch ],
        [ a owl:Restriction ;
            owl:allValuesFrom linkml:StructuredAlias ;
            owl:onProperty skosxl:altLabel ],
        [ a owl:Restriction ;
            owl:allValuesFrom linkml:Uriorcurie ;
            owl:onProperty skos:exactMatch ],
        [ a owl:Restriction ;
            owl:maxQualifiedCardinality 1 ;
            owl:onClass linkml:Uriorcurie ;
            owl:onProperty bibo:status ],
        [ a owl:Restriction ;
            owl:maxQualifiedCardinality 1 ;
            owl:onClass linkml:String ;
            owl:onProperty skos:definition ],
        [ a owl:Restriction ;
            owl:maxQualifiedCardinality 1 ;
            owl:onClass linkml:Uriorcurie ;
            owl:onProperty linkml:deprecated_element_has_possible_replacement ],
        [ a owl:Restriction ;
            owl:allValuesFrom linkml:String ;
            owl:onProperty skos:editorialNote ],
        [ a owl:Restriction ;
            owl:allValuesFrom linkml:SubsetDefinition ;
            owl:onProperty OIO:inSubset ],
        [ a owl:Restriction ;
            owl:allValuesFrom linkml:Example ;
            owl:onProperty linkml:examples ],
        [ a owl:Restriction ;
            owl:maxQualifiedCardinality 1 ;
            owl:onClass linkml:Uriorcurie ;
            owl:onProperty oslc:modifiedBy ],
        [ a owl:Restriction ;
            owl:allValuesFrom linkml:Annotation ;
            owl:onProperty linkml:annotations ],
        [ a owl:Restriction ;
            owl:maxQualifiedCardinality 1 ;
            owl:onClass linkml:Uriorcurie ;
            owl:onProperty dcterms:source ],
        [ a owl:Restriction ;
            owl:allValuesFrom linkml:String ;
            owl:onProperty linkml:todos ],
        [ a owl:Restriction ;
            owl:allValuesFrom linkml:AltDescription ;
            owl:onProperty linkml:alt_descriptions ],
        [ a owl:Restriction ;
            owl:allValuesFrom linkml:Extension ;
            owl:onProperty linkml:extensions ],
        [ a owl:Restriction ;
            owl:maxQualifiedCardinality 1 ;
            owl:onClass linkml:String ;
            owl:onProperty dcterms:title ],
        [ a owl:Restriction ;
            owl:maxQualifiedCardinality 1 ;
            owl:onClass linkml:Datetime ;
            owl:onProperty pav:lastUpdatedOn ],
        [ a owl:Restriction ;
            owl:allValuesFrom linkml:Uriorcurie ;
            owl:onProperty skos:mappingRelation ],
        [ a owl:Restriction ;
            owl:maxQualifiedCardinality 1 ;
            owl:onClass linkml:Integer ;
            owl:onProperty sh:order ],
        [ a owl:Restriction ;
            owl:maxQualifiedCardinality 1 ;
            owl:onClass linkml:AliasPredicateEnum ;
            owl:onProperty rdf:predicate ],
        [ a owl:Restriction ;
            owl:allValuesFrom linkml:Uriorcurie ;
            owl:onProperty skos:narrowMatch ],
        linkml:Annotatable,
        linkml:CommonMetadata,
        linkml:Expression,
        linkml:Extensible ;
    skos:definition "object that contains meta data about a synonym or alias including where it came from (source) and its scope (narrow, broad, etc.)" ;
    skos:exactMatch skosxl:Label .

linkml:SubsetDefinition a owl:Class,
        linkml:ClassDefinition ;
    rdfs:label "subset_definition" ;
    rdfs:subClassOf linkml:Element ;
    skos:definition "an element that can be used to group other metamodel elements" .

skos:exactMatch a owl:Class,
        owl:ObjectProperty,
        linkml:AliasPredicateEnum,
        linkml:SlotDefinition ;
    rdfs:label "EXACT_SYNONYM",
        "exact mappings" ;
    rdfs:range linkml:Uriorcurie ;
    rdfs:subPropertyOf skos:mappingRelation ;
    skos:definition "A list of terms from different schemas or terminology systems that have identical meaning." ;
    skos:exactMatch skos:exactMatch .

linkml:Example a owl:Class,
        linkml:ClassDefinition ;
    rdfs:label "example" ;
    rdfs:subClassOf [ a owl:Restriction ;
            owl:maxQualifiedCardinality 1 ;
            owl:onClass linkml:String ;
            owl:onProperty skos:example ],
        [ a owl:Restriction ;
            owl:maxQualifiedCardinality 1 ;
            owl:onClass linkml:String ;
            owl:onProperty linkml:description ],
        [ a owl:Restriction ;
            owl:maxQualifiedCardinality 1 ;
            owl:onClass linkml:Anything ;
            owl:onProperty linkml:object ] ;
    skos:definition "usage example and description" .

linkml:Extension a owl:Class,
        linkml:ClassDefinition ;
    rdfs:label "extension" ;
    rdfs:subClassOf [ a owl:Restriction ;
            owl:onClass linkml:String ;
            owl:onProperty linkml:value ;
            owl:qualifiedCardinality 1 ],
        [ a owl:Restriction ;
            owl:allValuesFrom linkml:Extension ;
            owl:onProperty linkml:extensions ],
        [ a owl:Restriction ;
            owl:onClass linkml:Uriorcurie ;
            owl:onProperty linkml:tag ;
            owl:qualifiedCardinality 1 ] ;
    skos:definition "a tag/value pair used to add non-model information to an entry" .

skos:mappingRelation a owl:ObjectProperty,
        linkml:SlotDefinition ;
    rdfs:label "mappings" ;
    rdfs:range linkml:Uriorcurie ;
    skos:altLabel "alternate identifiers",
        "alternate ids",
        "identifiers",
        "xrefs" ;
    skos:definition "A list of terms from different schemas or terminology systems that have comparable meaning. These may include terms that are precisely equivalent, broader or narrower in meaning, or otherwise semantically related but not equivalent from a strict ontological perspective." ;
    skos:exactMatch skos:mappingRelation .

linkml:EnumExpression a owl:Class,
        linkml:ClassDefinition ;
    rdfs:label "enum_expression" ;
    rdfs:subClassOf [ a owl:Restriction ;
            owl:allValuesFrom linkml:Uriorcurie ;
            owl:onProperty linkml:concepts ],
        [ a owl:Restriction ;
            owl:allValuesFrom linkml:AnonymousEnumExpression ;
            owl:onProperty linkml:include ],
        [ a owl:Restriction ;
            owl:allValuesFrom linkml:EnumDefinition ;
            owl:onProperty linkml:inherits ],
        [ a owl:Restriction ;
            owl:allValuesFrom linkml:AnonymousEnumExpression ;
            owl:onProperty linkml:minus ],
        [ a owl:Restriction ;
            owl:maxQualifiedCardinality 1 ;
            owl:onClass linkml:MatchQuery ;
            owl:onProperty linkml:matches ],
        [ a owl:Restriction ;
            owl:maxQualifiedCardinality 1 ;
            owl:onClass linkml:PvFormulaOptions ;
            owl:onProperty linkml:pv_formula ],
        [ a owl:Restriction ;
            owl:maxQualifiedCardinality 1 ;
            owl:onClass linkml:String ;
            owl:onProperty linkml:code_set_version ],
        [ a owl:Restriction ;
            owl:maxQualifiedCardinality 1 ;
            owl:onClass linkml:Uriorcurie ;
            owl:onProperty linkml:code_set ],
        [ a owl:Restriction ;
            owl:maxQualifiedCardinality 1 ;
            owl:onClass linkml:ReachabilityQuery ;
            owl:onProperty linkml:reachable_from ],
        [ a owl:Restriction ;
            owl:allValuesFrom linkml:PermissibleValue ;
            owl:onProperty linkml:permissible_values ],
        [ a owl:Restriction ;
            owl:maxQualifiedCardinality 1 ;
            owl:onClass linkml:String ;
            owl:onProperty linkml:code_set_tag ],
        linkml:Expression ;
    skos:definition "An expression that constrains the range of a slot" .

linkml:AnonymousSlotExpression a owl:Class,
        linkml:ClassDefinition ;
    rdfs:label "anonymous_slot_expression" ;
    rdfs:subClassOf [ a owl:Restriction ;
            owl:maxQualifiedCardinality 1 ;
            owl:onClass linkml:PresenceEnum ;
            owl:onProperty linkml:value_presence ],
        [ a owl:Restriction ;
            owl:maxQualifiedCardinality 1 ;
            owl:onClass linkml:Boolean ;
            owl:onProperty linkml:inlined ],
        [ a owl:Restriction ;
            owl:maxQualifiedCardinality 1 ;
            owl:onClass linkml:Boolean ;
            owl:onProperty linkml:recommended ],
        [ a owl:Restriction ;
            owl:maxQualifiedCardinality 1 ;
            owl:onClass linkml:AnonymousClassExpression ;
            owl:onProperty linkml:range_expression ],
        [ a owl:Restriction ;
            owl:maxQualifiedCardinality 1 ;
            owl:onClass linkml:EnumExpression ;
            owl:onProperty linkml:enum_range ],
        [ a owl:Restriction ;
            owl:maxQualifiedCardinality 1 ;
            owl:onClass linkml:AnonymousSlotExpression ;
            owl:onProperty linkml:has_member ],
        [ a owl:Restriction ;
            owl:maxQualifiedCardinality 1 ;
            owl:onClass linkml:String ;
            owl:onProperty linkml:implicit_prefix ],
        [ a owl:Restriction ;
            owl:maxQualifiedCardinality 1 ;
            owl:onClass linkml:Element ;
            owl:onProperty linkml:range ],
        [ a owl:Restriction ;
            owl:maxQualifiedCardinality 1 ;
            owl:onClass linkml:Integer ;
            owl:onProperty linkml:maximum_cardinality ],
        [ a owl:Restriction ;
            owl:maxQualifiedCardinality 1 ;
            owl:onClass linkml:String ;
            owl:onProperty linkml:pattern ],
        [ a owl:Restriction ;
            owl:allValuesFrom linkml:AnonymousSlotExpression ;
            owl:onProperty linkml:none_of ],
        [ a owl:Restriction ;
            owl:maxQualifiedCardinality 1 ;
            owl:onClass linkml:AnonymousSlotExpression ;
            owl:onProperty linkml:all_members ],
        [ a owl:Restriction ;
            owl:allValuesFrom linkml:AnonymousSlotExpression ;
            owl:onProperty linkml:exactly_one_of ],
        [ a owl:Restriction ;
            owl:allValuesFrom linkml:AnonymousSlotExpression ;
            owl:onProperty linkml:all_of ],
        [ a owl:Restriction ;
            owl:allValuesFrom linkml:String ;
            owl:onProperty linkml:equals_string_in ],
        [ a owl:Restriction ;
            owl:maxQualifiedCardinality 1 ;
            owl:onClass linkml:Boolean ;
            owl:onProperty linkml:required ],
        [ a owl:Restriction ;
            owl:maxQualifiedCardinality 1 ;
            owl:onClass linkml:Integer ;
            owl:onProperty linkml:minimum_cardinality ],
        [ a owl:Restriction ;
            owl:maxQualifiedCardinality 1 ;
            owl:onClass linkml:Integer ;
            owl:onProperty linkml:maximum_value ],
        [ a owl:Restriction ;
            owl:maxQualifiedCardinality 1 ;
            owl:onClass linkml:PatternExpression ;
            owl:onProperty linkml:structured_pattern ],
        [ a owl:Restriction ;
            owl:maxQualifiedCardinality 1 ;
            owl:onClass linkml:String ;
            owl:onProperty linkml:equals_expression ],
        [ a owl:Restriction ;
            owl:allValuesFrom linkml:AnonymousSlotExpression ;
            owl:onProperty linkml:any_of ],
        [ a owl:Restriction ;
            owl:maxQualifiedCardinality 1 ;
            owl:onClass linkml:Boolean ;
            owl:onProperty linkml:inlined_as_list ],
        [ a owl:Restriction ;
            owl:maxQualifiedCardinality 1 ;
            owl:onClass linkml:String ;
            owl:onProperty linkml:equals_string ],
        [ a owl:Restriction ;
            owl:maxQualifiedCardinality 1 ;
            owl:onClass linkml:UnitOfMeasure ;
            owl:onProperty qudt:unit ],
        [ a owl:Restriction ;
            owl:maxQualifiedCardinality 1 ;
            owl:onClass linkml:Integer ;
            owl:onProperty linkml:minimum_value ],
        [ a owl:Restriction ;
            owl:maxQualifiedCardinality 1 ;
            owl:onClass linkml:Integer ;
            owl:onProperty linkml:equals_number ],
        linkml:AnonymousExpression,
        linkml:SlotExpression .

linkml:SchemaDefinition a owl:Class,
        linkml:ClassDefinition ;
    rdfs:label "schema_definition" ;
    rdfs:seeAlso "https://en.wikipedia.org/wiki/Data_dictionary" ;
    rdfs:subClassOf [ a owl:Restriction ;
            owl:maxQualifiedCardinality 1 ;
            owl:onClass linkml:Datetime ;
            owl:onProperty linkml:source_file_date ],
        [ a owl:Restriction ;
            owl:allValuesFrom linkml:TypeDefinition ;
            owl:onProperty linkml:types ],
        [ a owl:Restriction ;
            owl:maxQualifiedCardinality 1 ;
            owl:onClass linkml:Datetime ;
            owl:onProperty linkml:generation_date ],
        [ a owl:Restriction ;
            owl:maxQualifiedCardinality 1 ;
            owl:onClass linkml:TypeDefinition ;
            owl:onProperty linkml:default_range ],
        [ a owl:Restriction ;
            owl:maxQualifiedCardinality 1 ;
            owl:onClass linkml:String ;
            owl:onProperty linkml:metamodel_version ],
        [ a owl:Restriction ;
            owl:allValuesFrom linkml:String ;
            owl:onProperty schema:keywords ],
        [ a owl:Restriction ;
            owl:maxQualifiedCardinality 1 ;
            owl:onClass linkml:String ;
            owl:onProperty dcterms:license ],
        [ a owl:Restriction ;
            owl:allValuesFrom linkml:EnumDefinition ;
            owl:onProperty linkml:enums ],
        [ a owl:Restriction ;
            owl:allValuesFrom linkml:SubsetDefinition ;
            owl:onProperty linkml:subsets ],
        [ a owl:Restriction ;
            owl:onClass linkml:Uri ;
            owl:onProperty linkml:id ;
            owl:qualifiedCardinality 1 ],
        [ a owl:Restriction ;
            owl:maxQualifiedCardinality 1 ;
            owl:onClass linkml:String ;
            owl:onProperty pav:version ],
        [ a owl:Restriction ;
            owl:allValuesFrom linkml:String ;
            owl:onProperty linkml:default_curi_maps ],
        [ a owl:Restriction ;
            owl:allValuesFrom linkml:Setting ;
            owl:onProperty linkml:settings ],
        [ a owl:Restriction ;
            owl:maxQualifiedCardinality 1 ;
            owl:onClass linkml:String ;
            owl:onProperty linkml:source_file ],
        [ a owl:Restriction ;
            owl:maxQualifiedCardinality 1 ;
            owl:onClass linkml:String ;
            owl:onProperty linkml:default_prefix ],
        [ a owl:Restriction ;
            owl:allValuesFrom linkml:Prefix ;
            owl:onProperty sh:declare ],
        [ a owl:Restriction ;
            owl:allValuesFrom linkml:Ncname ;
            owl:onProperty linkml:emit_prefixes ],
        [ a owl:Restriction ;
            owl:onClass linkml:Ncname ;
            owl:onProperty rdfs:label ;
            owl:qualifiedCardinality 1 ],
        [ a owl:Restriction ;
            owl:allValuesFrom linkml:ClassDefinition ;
            owl:onProperty linkml:classes ],
        [ a owl:Restriction ;
            owl:maxQualifiedCardinality 1 ;
            owl:onClass linkml:Integer ;
            owl:onProperty linkml:source_file_size ],
        [ a owl:Restriction ;
            owl:maxQualifiedCardinality 1 ;
            owl:onClass linkml:Boolean ;
            owl:onProperty linkml:slot_names_unique ],
        [ a owl:Restriction ;
            owl:allValuesFrom linkml:Uriorcurie ;
            owl:onProperty dcterms:subject ],
        [ a owl:Restriction ;
            owl:allValuesFrom linkml:SlotDefinition ;
            owl:onProperty linkml:slots ],
        [ a owl:Restriction ;
            owl:allValuesFrom linkml:Uriorcurie ;
            owl:onProperty linkml:imports ],
        linkml:Element ;
    skos:altLabel "data dictionary",
        "data model",
        "information model",
        "logical model",
        "model",
        "schema" ;
    skos:closeMatch qb:ComponentSet,
        owl:Ontology ;
    skos:definition "A collection of definitions that make up a schema or a data model." .

linkml:AnonymousClassExpression a owl:Class,
        linkml:ClassDefinition ;
    rdfs:label "anonymous_class_expression" ;
    rdfs:subClassOf [ a owl:Restriction ;
            owl:allValuesFrom linkml:AnonymousClassExpression ;
            owl:onProperty linkml:none_of ],
        [ a owl:Restriction ;
            owl:allValuesFrom linkml:AnonymousClassExpression ;
            owl:onProperty linkml:exactly_one_of ],
        [ a owl:Restriction ;
            owl:allValuesFrom linkml:AnonymousClassExpression ;
            owl:onProperty linkml:any_of ],
        [ a owl:Restriction ;
            owl:allValuesFrom linkml:SlotDefinition ;
            owl:onProperty linkml:slot_conditions ],
        [ a owl:Restriction ;
            owl:allValuesFrom linkml:AnonymousClassExpression ;
            owl:onProperty linkml:all_of ],
        [ a owl:Restriction ;
            owl:maxQualifiedCardinality 1 ;
            owl:onClass linkml:Definition ;
            owl:onProperty linkml:is_a ],
        linkml:AnonymousExpression,
        linkml:ClassExpression .

linkml:Definition a owl:Class,
        linkml:ClassDefinition ;
    rdfs:label "definition" ;
    rdfs:seeAlso "https://en.wikipedia.org/wiki/Data_element_definition" ;
    rdfs:subClassOf [ a owl:Restriction ;
            owl:maxQualifiedCardinality 1 ;
            owl:onClass linkml:Boolean ;
            owl:onProperty linkml:mixin ],
        [ a owl:Restriction ;
            owl:maxQualifiedCardinality 1 ;
            owl:onClass linkml:Boolean ;
            owl:onProperty linkml:abstract ],
        [ a owl:Restriction ;
            owl:allValuesFrom linkml:Definition ;
            owl:onProperty linkml:apply_to ],
        [ a owl:Restriction ;
            owl:maxQualifiedCardinality 1 ;
            owl:onClass linkml:String ;
            owl:onProperty linkml:string_serialization ],
        [ a owl:Restriction ;
            owl:maxQualifiedCardinality 1 ;
            owl:onClass linkml:Definition ;
            owl:onProperty linkml:is_a ],
        [ a owl:Restriction ;
            owl:allValuesFrom linkml:Uriorcurie ;
            owl:onProperty linkml:values_from ],
        [ a owl:Restriction ;
            owl:allValuesFrom linkml:Definition ;
            owl:onProperty linkml:mixins ],
        linkml:Element ;
    skos:definition "abstract base class for core metaclasses" .

linkml:Element a owl:Class,
        linkml:ClassDefinition ;
    rdfs:label "element" ;
    rdfs:seeAlso "https://en.wikipedia.org/wiki/Data_element" ;
    rdfs:subClassOf [ a owl:Restriction ;
            owl:maxQualifiedCardinality 1 ;
            owl:onClass linkml:Datetime ;
            owl:onProperty pav:createdOn ],
        [ a owl:Restriction ;
            owl:allValuesFrom linkml:Uriorcurie ;
            owl:onProperty skos:mappingRelation ],
        [ a owl:Restriction ;
            owl:allValuesFrom linkml:Uriorcurie ;
            owl:onProperty linkml:implements ],
        [ a owl:Restriction ;
            owl:allValuesFrom linkml:Uriorcurie ;
            owl:onProperty skos:broadMatch ],
        [ a owl:Restriction ;
            owl:maxQualifiedCardinality 1 ;
            owl:onClass linkml:String ;
            owl:onProperty skos:definition ],
        [ a owl:Restriction ;
            owl:allValuesFrom linkml:Annotation ;
            owl:onProperty linkml:annotations ],
        [ a owl:Restriction ;
            owl:maxQualifiedCardinality 1 ;
            owl:onClass linkml:Uriorcurie ;
            owl:onProperty bibo:status ],
        [ a owl:Restriction ;
            owl:allValuesFrom linkml:String ;
            owl:onProperty skos:editorialNote ],
        [ a owl:Restriction ;
            owl:maxQualifiedCardinality 1 ;
            owl:onClass linkml:String ;
            owl:onProperty linkml:imported_from ],
        [ a owl:Restriction ;
            owl:allValuesFrom linkml:Uriorcurie ;
            owl:onProperty skos:closeMatch ],
        [ a owl:Restriction ;
            owl:maxQualifiedCardinality 1 ;
            owl:onClass linkml:Uriorcurie ;
            owl:onProperty linkml:deprecated_element_has_exact_replacement ],
        [ a owl:Restriction ;
            owl:allValuesFrom linkml:StructuredAlias ;
            owl:onProperty skosxl:altLabel ],
        [ a owl:Restriction ;
            owl:allValuesFrom linkml:String ;
            owl:onProperty skos:note ],
        [ a owl:Restriction ;
            owl:allValuesFrom linkml:String ;
            owl:onProperty linkml:todos ],
        [ a owl:Restriction ;
            owl:maxQualifiedCardinality 1 ;
            owl:onClass linkml:Uriorcurie ;
            owl:onProperty dcterms:source ],
        [ a owl:Restriction ;
            owl:allValuesFrom linkml:Uriorcurie ;
            owl:onProperty skos:narrowMatch ],
        [ a owl:Restriction ;
            owl:onClass linkml:String ;
            owl:onProperty rdfs:label ;
            owl:qualifiedCardinality 1 ],
        [ a owl:Restriction ;
            owl:maxQualifiedCardinality 1 ;
            owl:onClass linkml:Integer ;
            owl:onProperty sh:order ],
        [ a owl:Restriction ;
            owl:maxQualifiedCardinality 1 ;
            owl:onClass linkml:Uriorcurie ;
            owl:onProperty oslc:modifiedBy ],
        [ a owl:Restriction ;
            owl:maxQualifiedCardinality 1 ;
            owl:onClass linkml:String ;
            owl:onProperty linkml:deprecated ],
        [ a owl:Restriction ;
            owl:maxQualifiedCardinality 1 ;
            owl:onClass linkml:Uri ;
            owl:onProperty skos:inScheme ],
        [ a owl:Restriction ;
            owl:maxQualifiedCardinality 1 ;
            owl:onClass linkml:Uriorcurie ;
            owl:onProperty linkml:deprecated_element_has_possible_replacement ],
        [ a owl:Restriction ;
            owl:allValuesFrom linkml:AltDescription ;
            owl:onProperty linkml:alt_descriptions ],
        [ a owl:Restriction ;
            owl:allValuesFrom linkml:Extension ;
            owl:onProperty linkml:extensions ],
        [ a owl:Restriction ;
            owl:maxQualifiedCardinality 1 ;
            owl:onClass linkml:String ;
            owl:onProperty schema:inLanguage ],
        [ a owl:Restriction ;
            owl:allValuesFrom linkml:Uriorcurie ;
            owl:onProperty skos:exactMatch ],
        [ a owl:Restriction ;
            owl:allValuesFrom linkml:Ncname ;
            owl:onProperty linkml:id_prefixes ],
        [ a owl:Restriction ;
            owl:allValuesFrom linkml:Example ;
            owl:onProperty linkml:examples ],
        [ a owl:Restriction ;
            owl:maxQualifiedCardinality 1 ;
            owl:onClass linkml:String ;
            owl:onProperty dcterms:title ],
        [ a owl:Restriction ;
            owl:maxQualifiedCardinality 1 ;
            owl:onClass linkml:String ;
            owl:onProperty dcterms:conformsTo ],
        [ a owl:Restriction ;
            owl:maxQualifiedCardinality 1 ;
            owl:onClass linkml:Datetime ;
            owl:onProperty pav:lastUpdatedOn ],
        [ a owl:Restriction ;
            owl:maxQualifiedCardinality 1 ;
            owl:onClass linkml:Uriorcurie ;
            owl:onProperty pav:createdBy ],
        [ a owl:Restriction ;
            owl:allValuesFrom linkml:String ;
            owl:onProperty skos:altLabel ],
        [ a owl:Restriction ;
            owl:allValuesFrom linkml:Uriorcurie ;
            owl:onProperty skos:relatedMatch ],
        [ a owl:Restriction ;
            owl:allValuesFrom linkml:LocalName ;
            owl:onProperty linkml:local_names ],
        [ a owl:Restriction ;
            owl:allValuesFrom linkml:SubsetDefinition ;
            owl:onProperty OIO:inSubset ],
        [ a owl:Restriction ;
            owl:maxQualifiedCardinality 1 ;
            owl:onClass linkml:Uriorcurie ;
            owl:onProperty linkml:definition_uri ],
        [ a owl:Restriction ;
            owl:allValuesFrom linkml:Uriorcurie ;
            owl:onProperty rdfs:seeAlso ],
        linkml:Annotatable,
        linkml:CommonMetadata,
        linkml:Extensible ;
    skos:altLabel "data element",
        "object" ;
    skos:definition "A named element in the model" .

linkml:ClassDefinition a owl:Class,
        linkml:ClassDefinition ;
    rdfs:label "class_definition" ;
    rdfs:subClassOf [ a owl:Restriction ;
            owl:allValuesFrom linkml:AnonymousClassExpression ;
            owl:onProperty linkml:exactly_one_of ],
        [ a owl:Restriction ;
            owl:allValuesFrom linkml:ClassDefinition ;
            owl:onProperty linkml:mixins ],
        [ a owl:Restriction ;
            owl:allValuesFrom linkml:SlotDefinition ;
            owl:onProperty linkml:slots ],
        [ a owl:Restriction ;
            owl:allValuesFrom linkml:UniqueKey ;
            owl:onProperty linkml:unique_keys ],
        [ a owl:Restriction ;
            owl:maxQualifiedCardinality 1 ;
            owl:onClass linkml:Uriorcurie ;
            owl:onProperty linkml:subclass_of ],
        [ a owl:Restriction ;
            owl:allValuesFrom linkml:SlotDefinition ;
            owl:onProperty linkml:slot_conditions ],
        [ a owl:Restriction ;
            owl:allValuesFrom linkml:AnonymousClassExpression ;
            owl:onProperty linkml:classification_rules ],
        [ a owl:Restriction ;
            owl:maxQualifiedCardinality 1 ;
            owl:onClass linkml:Boolean ;
            owl:onProperty linkml:tree_root ],
        [ a owl:Restriction ;
            owl:maxQualifiedCardinality 1 ;
            owl:onClass linkml:Boolean ;
            owl:onProperty linkml:children_are_mutually_disjoint ],
        [ a owl:Restriction ;
            owl:allValuesFrom linkml:AnonymousClassExpression ;
            owl:onProperty linkml:any_of ],
        [ a owl:Restriction ;
            owl:allValuesFrom linkml:AnonymousClassExpression ;
            owl:onProperty linkml:all_of ],
        [ a owl:Restriction ;
            owl:allValuesFrom linkml:ClassDefinition ;
            owl:onProperty linkml:union_of ],
        [ a owl:Restriction ;
            owl:allValuesFrom linkml:AnonymousClassExpression ;
            owl:onProperty linkml:none_of ],
        [ a owl:Restriction ;
            owl:allValuesFrom linkml:SlotDefinition ;
            owl:onProperty linkml:slot_usage ],
        [ a owl:Restriction ;
            owl:allValuesFrom linkml:SlotDefinition ;
            owl:onProperty linkml:defining_slots ],
        [ a owl:Restriction ;
            owl:allValuesFrom linkml:ClassDefinition ;
            owl:onProperty linkml:disjoint_with ],
        [ a owl:Restriction ;
            owl:maxQualifiedCardinality 1 ;
            owl:onClass linkml:Boolean ;
            owl:onProperty linkml:represents_relationship ],
        [ a owl:Restriction ;
            owl:allValuesFrom linkml:ClassRule ;
            owl:onProperty sh:rule ],
        [ a owl:Restriction ;
            owl:allValuesFrom linkml:SlotDefinition ;
            owl:onProperty linkml:attributes ],
        [ a owl:Restriction ;
            owl:allValuesFrom linkml:ClassDefinition ;
            owl:onProperty linkml:apply_to ],
        [ a owl:Restriction ;
            owl:maxQualifiedCardinality 1 ;
            owl:onClass linkml:Uriorcurie ;
            owl:onProperty linkml:class_uri ],
        [ a owl:Restriction ;
            owl:maxQualifiedCardinality 1 ;
            owl:onClass linkml:ClassDefinition ;
            owl:onProperty linkml:is_a ],
        [ a owl:Restriction ;
            owl:maxQualifiedCardinality 1 ;
            owl:onClass linkml:Boolean ;
            owl:onProperty linkml:slot_names_unique ],
        linkml:ClassExpression,
        linkml:Definition ;
    skos:altLabel "message",
        "observation",
        "record",
        "table",
        "template" ;
    skos:closeMatch owl:Class ;
    skos:definition "an element whose instances are complex objects that may have slot-value assignments" .

linkml:SlotDefinition a owl:Class,
        linkml:ClassDefinition ;
    rdfs:label "slot_definition" ;
    rdfs:subClassOf [ a owl:Restriction ;
            owl:maxQualifiedCardinality 1 ;
            owl:onClass linkml:ClassDefinition ;
            owl:onProperty linkml:domain ],
        [ a owl:Restriction ;
            owl:maxQualifiedCardinality 1 ;
            owl:onClass linkml:String ;
            owl:onProperty linkml:pattern ],
        [ a owl:Restriction ;
            owl:maxQualifiedCardinality 1 ;
            owl:onClass linkml:Boolean ;
            owl:onProperty linkml:inherited ],
        [ a owl:Restriction ;
            owl:maxQualifiedCardinality 1 ;
            owl:onClass linkml:Boolean ;
            owl:onProperty linkml:recommended ],
        [ a owl:Restriction ;
            owl:maxQualifiedCardinality 1 ;
            owl:onClass linkml:Integer ;
            owl:onProperty linkml:maximum_cardinality ],
        [ a owl:Restriction ;
            owl:maxQualifiedCardinality 1 ;
            owl:onClass linkml:Boolean ;
            owl:onProperty linkml:required ],
        [ a owl:Restriction ;
            owl:maxQualifiedCardinality 1 ;
            owl:onClass linkml:Boolean ;
            owl:onProperty linkml:is_grouping_slot ],
        [ a owl:Restriction ;
            owl:maxQualifiedCardinality 1 ;
            owl:onClass linkml:Boolean ;
            owl:onProperty linkml:inlined_as_list ],
        [ a owl:Restriction ;
            owl:maxQualifiedCardinality 1 ;
            owl:onClass linkml:Integer ;
            owl:onProperty linkml:equals_number ],
        [ a owl:Restriction ;
            owl:maxQualifiedCardinality 1 ;
            owl:onClass linkml:Boolean ;
            owl:onProperty linkml:symmetric ],
        [ a owl:Restriction ;
            owl:allValuesFrom linkml:AnonymousSlotExpression ;
            owl:onProperty linkml:all_of ],
        [ a owl:Restriction ;
            owl:maxQualifiedCardinality 1 ;
            owl:onClass linkml:PathExpression ;
            owl:onProperty linkml:path_rule ],
        [ a owl:Restriction ;
            owl:allValuesFrom linkml:SlotDefinition ;
            owl:onProperty linkml:mixins ],
        [ a owl:Restriction ;
            owl:allValuesFrom linkml:SlotDefinition ;
            owl:onProperty linkml:disjoint_with ],
        [ a owl:Restriction ;
            owl:maxQualifiedCardinality 1 ;
            owl:onClass linkml:Boolean ;
            owl:onProperty linkml:children_are_mutually_disjoint ],
        [ a owl:Restriction ;
            owl:maxQualifiedCardinality 1 ;
            owl:onClass linkml:Integer ;
            owl:onProperty linkml:minimum_value ],
        [ a owl:Restriction ;
            owl:maxQualifiedCardinality 1 ;
            owl:onClass linkml:RelationalRoleEnum ;
            owl:onProperty linkml:relational_role ],
        [ a owl:Restriction ;
            owl:maxQualifiedCardinality 1 ;
            owl:onClass linkml:SlotDefinition ;
            owl:onProperty owl:inverseOf ],
        [ a owl:Restriction ;
            owl:maxQualifiedCardinality 1 ;
            owl:onClass linkml:String ;
            owl:onProperty linkml:usage_slot_name ],
        [ a owl:Restriction ;
            owl:maxQualifiedCardinality 1 ;
            owl:onClass linkml:String ;
            owl:onProperty linkml:ifabsent ],
        [ a owl:Restriction ;
            owl:maxQualifiedCardinality 1 ;
            owl:onClass linkml:PresenceEnum ;
            owl:onProperty linkml:value_presence ],
        [ a owl:Restriction ;
            owl:maxQualifiedCardinality 1 ;
            owl:onClass linkml:Integer ;
            owl:onProperty linkml:minimum_cardinality ],
        [ a owl:Restriction ;
            owl:maxQualifiedCardinality 1 ;
            owl:onClass linkml:String ;
            owl:onProperty linkml:equals_expression ],
        [ a owl:Restriction ;
            owl:maxQualifiedCardinality 1 ;
            owl:onClass linkml:Boolean ;
            owl:onProperty linkml:is_usage_slot ],
        [ a owl:Restriction ;
            owl:maxQualifiedCardinality 1 ;
            owl:onClass linkml:Boolean ;
            owl:onProperty linkml:designates_type ],
        [ a owl:Restriction ;
            owl:maxQualifiedCardinality 1 ;
            owl:onClass linkml:AnonymousSlotExpression ;
            owl:onProperty linkml:has_member ],
        [ a owl:Restriction ;
            owl:maxQualifiedCardinality 1 ;
            owl:onClass linkml:String ;
            owl:onProperty linkml:implicit_prefix ],
        [ a owl:Restriction ;
            owl:maxQualifiedCardinality 1 ;
            owl:onClass linkml:Boolean ;
            owl:onProperty linkml:inlined ],
        [ a owl:Restriction ;
            owl:maxQualifiedCardinality 1 ;
            owl:onClass linkml:SlotDefinition ;
            owl:onProperty linkml:reflexive_transitive_form_of ],
        [ a owl:Restriction ;
            owl:maxQualifiedCardinality 1 ;
            owl:onClass linkml:Boolean ;
            owl:onProperty linkml:reflexive ],
        [ a owl:Restriction ;
            owl:maxQualifiedCardinality 1 ;
            owl:onClass linkml:String ;
            owl:onProperty linkml:singular_name ],
        [ a owl:Restriction ;
            owl:allValuesFrom linkml:AnonymousSlotExpression ;
            owl:onProperty linkml:any_of ],
        [ a owl:Restriction ;
            owl:maxQualifiedCardinality 1 ;
            owl:onClass linkml:SlotDefinition ;
            owl:onProperty linkml:is_a ],
        [ a owl:Restriction ;
            owl:maxQualifiedCardinality 1 ;
            owl:onClass linkml:Boolean ;
            owl:onProperty linkml:locally_reflexive ],
        [ a owl:Restriction ;
            owl:maxQualifiedCardinality 1 ;
            owl:onClass linkml:Boolean ;
            owl:onProperty linkml:shared ],
        [ a owl:Restriction ;
            owl:maxQualifiedCardinality 1 ;
            owl:onClass linkml:AnonymousSlotExpression ;
            owl:onProperty linkml:all_members ],
        [ a owl:Restriction ;
            owl:maxQualifiedCardinality 1 ;
            owl:onClass linkml:Boolean ;
            owl:onProperty linkml:multivalued ],
        [ a owl:Restriction ;
            owl:allValuesFrom linkml:SlotDefinition ;
            owl:onProperty linkml:union_of ],
        [ a owl:Restriction ;
            owl:maxQualifiedCardinality 1 ;
            owl:onClass linkml:Boolean ;
            owl:onProperty linkml:key ],
        [ a owl:Restriction ;
            owl:maxQualifiedCardinality 1 ;
            owl:onClass linkml:String ;
            owl:onProperty linkml:role ],
        [ a owl:Restriction ;
            owl:allValuesFrom linkml:AnonymousSlotExpression ;
            owl:onProperty linkml:none_of ],
        [ a owl:Restriction ;
            owl:maxQualifiedCardinality 1 ;
            owl:onClass linkml:String ;
            owl:onProperty linkml:equals_string ],
        [ a owl:Restriction ;
            owl:maxQualifiedCardinality 1 ;
            owl:onClass linkml:AnonymousClassExpression ;
            owl:onProperty linkml:range_expression ],
        [ a owl:Restriction ;
            owl:maxQualifiedCardinality 1 ;
            owl:onClass linkml:Integer ;
            owl:onProperty linkml:maximum_value ],
        [ a owl:Restriction ;
            owl:maxQualifiedCardinality 1 ;
            owl:onClass linkml:SlotDefinition ;
            owl:onProperty linkml:transitive_form_of ],
        [ a owl:Restriction ;
            owl:maxQualifiedCardinality 1 ;
            owl:onClass linkml:Boolean ;
            owl:onProperty linkml:asymmetric ],
        [ a owl:Restriction ;
            owl:allValuesFrom linkml:ClassDefinition ;
            owl:onProperty linkml:domain_of ],
        [ a owl:Restriction ;
            owl:maxQualifiedCardinality 1 ;
            owl:onClass linkml:Boolean ;
            owl:onProperty linkml:list_elements_ordered ],
        [ a owl:Restriction ;
            owl:allValuesFrom linkml:String ;
            owl:onProperty linkml:equals_string_in ],
        [ a owl:Restriction ;
            owl:maxQualifiedCardinality 1 ;
            owl:onClass linkml:String ;
            owl:onProperty skos:prefLabel ],
        [ a owl:Restriction ;
            owl:maxQualifiedCardinality 1 ;
            owl:onClass linkml:Element ;
            owl:onProperty linkml:range ],
        [ a owl:Restriction ;
            owl:maxQualifiedCardinality 1 ;
            owl:onClass linkml:SlotDefinition ;
            owl:onProperty rdfs:subPropertyOf ],
        [ a owl:Restriction ;
            owl:maxQualifiedCardinality 1 ;
            owl:onClass linkml:Boolean ;
            owl:onProperty linkml:identifier ],
        [ a owl:Restriction ;
            owl:maxQualifiedCardinality 1 ;
            owl:onClass linkml:UnitOfMeasure ;
            owl:onProperty qudt:unit ],
        [ a owl:Restriction ;
            owl:maxQualifiedCardinality 1 ;
            owl:onClass linkml:EnumExpression ;
            owl:onProperty linkml:enum_range ],
        [ a owl:Restriction ;
            owl:maxQualifiedCardinality 1 ;
            owl:onClass linkml:Boolean ;
            owl:onProperty linkml:transitive ],
        [ a owl:Restriction ;
            owl:maxQualifiedCardinality 1 ;
            owl:onClass linkml:Boolean ;
            owl:onProperty linkml:is_class_field ],
        [ a owl:Restriction ;
            owl:maxQualifiedCardinality 1 ;
            owl:onClass linkml:Boolean ;
            owl:onProperty linkml:irreflexive ],
        [ a owl:Restriction ;
            owl:maxQualifiedCardinality 1 ;
            owl:onClass linkml:Definition ;
            owl:onProperty linkml:owner ],
        [ a owl:Restriction ;
            owl:maxQualifiedCardinality 1 ;
            owl:onClass linkml:Uriorcurie ;
            owl:onProperty linkml:slot_uri ],
        [ a owl:Restriction ;
            owl:allValuesFrom linkml:SlotDefinition ;
            owl:onProperty linkml:apply_to ],
        [ a owl:Restriction ;
            owl:maxQualifiedCardinality 1 ;
            owl:onClass linkml:PatternExpression ;
            owl:onProperty linkml:structured_pattern ],
        [ a owl:Restriction ;
            owl:maxQualifiedCardinality 1 ;
            owl:onClass linkml:SlotDefinition ;
            owl:onProperty sh:group ],
        [ a owl:Restriction ;
            owl:maxQualifiedCardinality 1 ;
            owl:onClass linkml:Boolean ;
            owl:onProperty linkml:list_elements_unique ],
        [ a owl:Restriction ;
            owl:maxQualifiedCardinality 1 ;
            owl:onClass linkml:String ;
            owl:onProperty linkml:readonly ],
        [ a owl:Restriction ;
            owl:allValuesFrom linkml:AnonymousSlotExpression ;
            owl:onProperty linkml:exactly_one_of ],
        linkml:Definition,
        linkml:SlotExpression ;
    skos:altLabel "attribute",
        "column",
        "field",
        "property",
        "slot",
        "variable" ;
    skos:closeMatch qb:ComponentProperty,
        rdf:Property ;
    skos:definition "an element that describes how instances are related to other instances" .


